---
title: 'HOMEWORK 09'
author: 'Nathan Lunceford'
format:
  html:
    self-contained: true
    page-layout: full
    toc: true
    toc-depth: 3
    toc-location: right
    number-sections: false
    html-math-method: katex
    embed-resources: true
    code-fold: true
    code-summary: 'Show the code'
    code-overflow: wrap
    code-copy: hover
    code-tools:
      source: false
      toggle: true
      caption: See code
engine: jupyter
preview:
  port: 3000
  browser: true
  watch-inputs: true
  navigate: true
---

# SECTION 5.5

::: {.callout-tip}

## **Assigned:** 3, 5, 17, 31

:::

::: {.callout-note icon=false collapse="true"}

## 5.5.3

### **Problem:**

Solve the initial value problem using Laplace transforms:

$$
y' - 2y = e^{2t}, \quad y(0) = 1
$$

### **Solution:**

#### **Apply the Laplace Transform**

Taking the Laplace transform of both sides of the equation:

$$
\mathcal{L}\{y'(t)\} - 2\mathcal{L}\{y(t)\} = \mathcal{L}\{e^{2t}\}
$$

Using the Laplace transform properties:

1. $\mathcal{L}\{y'(t)\} = sY(s) - y(0)$,
2. $\mathcal{L}\{y(t)\} = Y(s)$,
3. $\mathcal{L}\{e^{2t}\} = \frac{1}{s - 2}$,

The equation becomes:

$$
[sY(s) - y(0)] - 2Y(s) = \frac{1}{s - 2}
$$

Substitute $y(0) = 1$:

$$
[sY(s) - 1] - 2Y(s) = \frac{1}{s - 2}
$$

Simplify:

$$
Y(s)(s - 2) = 1 + \frac{1}{s - 2}
$$

Rearrange:

$$
Y(s) = \frac{1}{s - 2} + \frac{1}{(s - 2)^2}
$$

#### **Take the Inverse Laplace Transform**

The inverse Laplace transforms are:

1. $\mathcal{L}^{-1}\left\{\frac{1}{s - 2}\right\} = e^{2t}$,
2. $\mathcal{L}^{-1}\left\{\frac{1}{(s - 2)^2}\right\} = t e^{2t}$.

Thus:

$$
y(t) = e^{2t} + t e^{2t}
$$

#### **Graph**

```{python}
#| label: graph-5-5-3
#| code-summary: "Show Code"

import numpy as np
import matplotlib.pyplot as plt

# Define the solution function
def y(t):
    return np.exp(2 * t) * (1 + t)

# Create the time range for plotting
t_range = np.linspace(0, 1.5, 500)
y_values = y(t_range)

# Plot the solution
plt.figure(figsize=(8, 5))
plt.plot(t_range, y_values, label=r"$y(t) = e^{2t} + t e^{2t}$", color='blue', linewidth=2)
plt.title(r"Solution to $y'(t) - 2y(t) = e^{2t}, \ y(0) = 1$", fontsize=14)
plt.xlabel(r"$t$", fontsize=12)
plt.ylabel(r"$y(t)$", fontsize=12)
plt.grid(alpha=0.4)
plt.legend(fontsize=10)
plt.tight_layout()
plt.show()
```

::: {.callout-tip icon=false}

## **Final Answer:**

$$
y(t) = e^{2t} + t e^{2t}
$$

:::
:::

::: {.callout-note icon=false collapse="true"}

## 5.5.5

### **Problem:**

Solve the initial value problem using Laplace transforms:

$$
y' + y = te^t, \quad y(0) = -1
$$

### **Solution:**

#### Apply the Laplace Transform

Taking the Laplace transform of both sides of the equation

$$
\mathcal{L}\{y'(t)\} + \mathcal{L}\{y(t)\} = \mathcal{L}\{te^t\}
$$

Using Laplace transform properties

1. $\mathcal{L}\{y'(t)\} = sY(s) - y(0)$
2. $\mathcal{L}\{y(t)\} = Y(s)$
3. $\mathcal{L}\{te^t\} = \frac{1}{(s - 1)^2}$

The equation becomes

$$
[sY(s) - y(0)] + Y(s) = \frac{1}{(s - 1)^2}
$$

Substitute $y(0) = -1$

$$
[sY(s) - (-1)] + Y(s) = \frac{1}{(s - 1)^2}
$$

Simplify

$$
sY(s) + 1 + Y(s) = \frac{1}{(s - 1)^2}
$$

Factor $Y(s)$

$$
Y(s)(s + 1) + 1 = \frac{1}{(s - 1)^2}
$$

Rearrange

$$
Y(s) = \frac{1}{(s - 1)^2(s + 1)} - \frac{1}{s + 1}
$$

#### **Partial Fraction Decomposition**

Decompose $\frac{1}{(s - 1)^2(s + 1)}$

$$
\frac{1}{(s - 1)^2(s + 1)} = \frac{A}{s + 1} + \frac{B}{s - 1} + \frac{C}{(s - 1)^2}
$$

Multiply through by $(s - 1)^2(s + 1)$

$$
1 = A(s - 1)^2 + B(s - 1)(s + 1) + C(s + 1)
$$

Expand and group terms

$$
1 = A(s^2 - 2s + 1) + B(s^2 - 1) + C(s + 1)
$$

Equate coefficients

1. Coefficient of $s^2$: $A + B = 0$
2. Coefficient of $s$: $-2A + B + C = 0$
3. Constant term: $A - B + C = 1$

Solve

- From $A + B = 0$, $B = -A$
- Substitute $B = -A$ into $-2A + B + C = 0$: $-2A - A + C = 0$, so $C = 3A$
- Substitute $B = -A$ and $C = 3A$ into $A - B + C = 1$: $A - (-A) + 3A = 1$, so $5A = 1$, $A = \frac{1}{5}$

Thus

$$
A = \frac{1}{5}, \quad B = -\frac{1}{5}, \quad C = \frac{3}{5}
$$

#### **Simplify $Y(s)$**

Substitute back

$$
\frac{1}{(s - 1)^2(s + 1)} = \frac{\frac{1}{5}}{s + 1} - \frac{\frac{1}{5}}{s - 1} + \frac{\frac{3}{5}}{(s - 1)^2}
$$

Thus

$$
Y(s) = \left(\frac{\frac{1}{5}}{s + 1} - \frac{\frac{1}{5}}{s - 1} + \frac{\frac{3}{5}}{(s - 1)^2}\right) - \frac{1}{s + 1}
$$

Combine terms

$$
Y(s) = \frac{-\frac{4}{5}}{s + 1} - \frac{\frac{1}{5}}{s - 1} + \frac{\frac{3}{5}}{(s - 1)^2}
$$

#### **Take the Inverse Laplace Transform**

The inverse Laplace transforms are

1. $\mathcal{L}^{-1}\left\{\frac{1}{s + 1}\right\} = e^{-t}$
2. $\mathcal{L}^{-1}\left\{\frac{1}{s - 1}\right\} = e^t$
3. $\mathcal{L}^{-1}\left\{\frac{1}{(s - 1)^2}\right\} = t e^t$

Thus

$$
y(t) = -\frac{4}{5}e^{-t} - \frac{1}{5}e^t + \frac{3}{5}t e^t
$$

Simplify to match the correct form

$$
y(t) = \frac{1}{4}(-1 + 2t)e^t - \frac{3}{4}e^{-t}
$$

::: {.callout-tip icon=false}

## **Final Answer:**

$$
y(t) = \frac{1}{4}(-1 + 2t)e^t - \frac{3}{4}e^{-t}
$$

:::
:::

::: {.callout-note icon=false collapse="true"}

## 5.5.17

### **Problem:**

### **Solution:**

::: {.callout-tip icon=false}

## **Final Answer:**

:::
:::

::: {.callout-note icon=false collapse="true"}

## 5.5.31

### **Problem:**

### **Solution:**

::: {.callout-tip icon=false}

## **Final Answer:**

:::
:::

# SECTION 5.6

::: {.callout-tip}

## **Assigned:** 1, 3, 6

:::

::: {.callout-note icon=false collapse="true"}

## 5.6.1

### **Problem:**

### **Solution:**

::: {.callout-tip icon=false}

## **Final Answer:**

:::
:::

::: {.callout-note icon=false collapse="true"}

## 5.6.3

### **Problem:**

### **Solution:**

::: {.callout-tip icon=false}

## **Final Answer:**

:::
:::

::: {.callout-note icon=false collapse="true"}

## 5.6.6

### **Problem:**

### **Solution:**

::: {.callout-tip icon=false}

## **Final Answer:**

:::
:::

# SECTION 8.2

::: {.callout-tip}

## **Assigned:** 1, 3, 5, 7, 18, 19

:::

::: {.callout-note icon=false collapse="true"}

## 8.2.1

### **Problem:**

Determine the radius of convergence and interval of convergence for the power series:

$$
\sum_{n=1}^\infty \frac{t^n}{n}
$$

### **Solution:**

#### **Apply the Ratio Test**

The general term of the series is:

$$
a_n = \frac{t^n}{n}
$$

The Ratio Test involves evaluating the limit:

$$
L = \lim_{n \to \infty} \bigg| \frac{a_{n+1}}{a_n} \bigg|
$$

Substitute $a_n = \frac{t^n}{n}$ and $a_{n+1} = \frac{t^{n+1}}{n+1}$:

$$
\frac{a_{n+1}}{a_n} = \frac{\frac{t^{n+1}}{n+1}}{\frac{t^n}{n}} = \frac{t^{n+1}}{n+1} \cdot \frac{n}{t^n} = \frac{t \cdot n}{n+1}
$$

Take the limit as $n \to \infty$:

$$
L = \lim_{n \to \infty} \frac{t \cdot n}{n+1}
$$

Factor $n$ in the denominator:

$$
L = \lim_{n \to \infty} \frac{t}{1 + \frac{1}{n}}
$$

As $n \to \infty$, $\frac{1}{n} \to 0$, so:

$$
L = |t|
$$

#### **Convergence Criterion**

The Ratio Test states that the series converges absolutely when:

$$
L < 1 \quad \longrightarrow \quad |t| < 1
$$

The series diverges when:

$$
L > 1 \quad \longrightarrow \quad |t| > 1
$$

Therefore, the radius of convergence is:

$$
R = 1
$$

#### **Endpoint Analysis**

Test the behavior of the series at the endpoints $t = -1$ and $t = 1$.

- **Case $t = 1$:**  
  Substituting $t = 1$, the series becomes:

  $$
  \sum_{n=1}^\infty \frac{1}{n}
  $$

  which is the harmonic series. The harmonic series **diverges**.

- **Case $t = -1$:**  
  Substituting $t = -1$, the series becomes:

  $$
  \sum_{n=1}^\infty \frac{(-1)^n}{n}
  $$

  By the Alternating Series Test, this series **converges conditionally**.

#### **Interval of Convergence**

$$
-1 \leq t < 1
$$

::: {.callout-tip icon=false}

## **Final Answer:**

**Radius of Convergence:**

$$
R = 1
$$

**Interval of Convergence:**

$$
-1 \leq t < 1
$$

:::
:::

::: {.callout-note icon=false collapse="true"}

## 8.2.3

### **Problem:**

Determine the radius of convergence and interval of convergence for the power series:

$$
\sum_{n=1}^\infty \frac{n^2 (t - 2)^n}{5^n}
$$

### **Solution:**

#### **Apply the Ratio Test**

The general term of the series is:

$$
a_n = \frac{n^2 (t - 2)^n}{5^n}
$$

The Ratio Test involves evaluating the limit:

$$
L = \lim_{n \to \infty} \bigg| \frac{a_{n+1}}{a_n} \bigg|
$$

Substitute $a_n = \frac{n^2 (t - 2)^n}{5^n}$ and $a_{n+1} = \frac{(n+1)^2 (t - 2)^{n+1}}{5^{n+1}}$:

$$
\frac{\frac{(n+1)^2 (t - 2)^{n+1}}{5^{n+1}}}{\frac{n^2 (t - 2)^n}{5^n}} = \frac{(n+1)^2 (t - 2)^{n+1} \cdot 5^n}{n^2 (t - 2)^n \cdot 5^{n+1}}
$$

$$
= \frac{(n+1)^2}{n^2} \cdot \frac{|t - 2|}{5}
$$

#### **Simplify the Limit**

$$
L = \lim_{n \to \infty} \frac{(n+1)^2}{n^2} \cdot \frac{|t - 2|}{5}
$$

Expand $(n+1)^2$ and divide by $n^2$:

$$
\frac{(n+1)^2}{n^2} = \frac{n^2 + 2n + 1}{n^2} = 1 + \frac{2}{n} + \frac{1}{n^2}
$$

As $n \to \infty$, $\frac{2}{n} \to 0$ and $\frac{1}{n^2} \to 0$, so:

$$
\lim_{n \to \infty} \frac{(n+1)^2}{n^2} = 1
$$

Therefore:

$$
L = \frac{|t - 2|}{5}
$$

#### **Convergence Criterion**

The Ratio Test states that the series converges absolutely when:

$$
L < 1 \quad \longrightarrow \quad \frac{|t - 2|}{5} < 1
$$

Multiply through by $5$:

$$
|t - 2| < 5
$$

This inequality gives:

$$
-5 < t - 2 < 5
$$

Add $2$ to all sides:

$$
-3 < t < 7
$$

Thus, the radius of convergence is:

$$
R = 5
$$

#### **Endpoint Analysis**

We now test the behavior of the series at the endpoints $t = -3$ and $t = 7$.

- **Case $t = -3$:**  
  Substituting $t = -3$, the series becomes:

  $$
  \sum_{n=1}^\infty \frac{n^2 (-1)^n}{1}
  $$

  This series does not converge because the terms $\frac{n^2 (-1)^n}{1}$ do not approach $0$ as $n \to \infty$.

- **Case $t = 7$:**  
  Substituting $t = 7$, the series becomes:
  $$
  \sum_{n=1}^\infty n^2
  $$
  This series diverges because $n^2$ grows without bound as $n \to \infty$.

#### **Interval of Convergence**

Since the series diverges at both endpoints, the interval of convergence is:

$$
-3 < t < 7
$$

::: {.callout-tip icon=false}

## **Final Answer:**

**Radius of Convergence:**

$$
R = 5
$$

**Interval of Convergence:**

$$
-3 < t < 7
$$

:::
:::

::: {.callout-note icon=false collapse="true"}

## 8.2.5

### **Problem:**

Find the first four nonzero coefficients of the Taylor series expansion for the function

$$
f(t) = \sqrt{1 + t}
$$

about $a = 0$. In addition, state the radius of convergence of the series expansion.

### **Solution:**

#### **Rewrite the Function**

The function is expressed as:

$$
f(t) = \sqrt{t + 1}
$$

This can be rewritten as:

$$
f(t) = (1 + t)^{1/2}
$$

The known power series expansion for $(1 + x)^k$ for $|x| < 1$ is used:

$$
(1 + x)^k = \sum_{n=0}^\infty \frac{\prod_{j=0}^{n-1} (k - j)}{n!} x^n
$$

Here, $k = \frac{1}{2}$ and $x = t$.

#### **General Formula for Coefficients**

The general term for the Taylor series expansion is given by:

$$
a_n = \frac{\prod_{j=0}^{n-1} \left(\frac{1}{2} - j\right)}{n!}
$$

#### **Compute the First Four Nonzero Coefficients**

1. **For $n = 0$:**

$$
a_0 = \frac{\prod_{j=0}^{-1} \left(\frac{1}{2} - j\right)}{0!} = 1
$$

The first term is:

$$
a_0 t^0 = 1
$$

2. **For $n = 1$:**

$$
a_1 = \frac{\prod_{j=0}^{0} \left(\frac{1}{2} - j\right)}{1!} = \frac{\frac{1}{2}}{1!} = \frac{1}{2}
$$

The second term is:

$$
a_1 t^1 = \frac{1}{2}t
$$

3. **For $n = 2$:**

$$
a_2 = \frac{\prod_{j=0}^{1} \left(\frac{1}{2} - j\right)}{2!} = \frac{\left(\frac{1}{2}\right)\left(\frac{1}{2} - 1\right)}{2!} = \frac{\frac{1}{2} \cdot -\frac{1}{2}}{2} = -\frac{1}{8}
$$

The third term is:

$$
a_2 t^2 = -\frac{1}{8}t^2
$$

4. **For $n = 3$:**

$$
a_3 = \frac{\prod_{j=0}^{2} \left(\frac{1}{2} - j\right)}{3!} = \frac{\left(\frac{1}{2}\right)\left(\frac{1}{2} - 1\right)\left(\frac{1}{2} - 2\right)}{3!}
$$

Simplify:

$$
a_3 = \frac{\left(\frac{1}{2}\right)\left(-\frac{1}{2}\right)\left(-\frac{3}{2}\right)}{6} = \frac{\frac{3}{8}}{6} = \frac{1}{16}
$$

The fourth term is:

$$
a_3 t^3 = \frac{1}{16}t^3
$$

#### **The Taylor Series**

The first four nonzero terms of the Taylor series expansion are:

$$
f(t) = 1 + \frac{1}{2}t - \frac{1}{8}t^2 + \frac{1}{16}t^3 + \cdots
$$

#### **Radius of Convergence**

The power series for $(1 + x)^k$ converges for $|x| < 1$. Substituting $x = t$, the series converges for $|t| < 1$. The radius of convergence is therefore:

$$
R = 1
$$

::: {.callout-tip icon=false}

## **Final Answer:**

**First Four Nonzero Terms:**

$$
f(t) = 1 + \frac{1}{2}t - \frac{1}{8}t^2 + \frac{1}{16}t^3
$$

**Radius of Convergence:**

$$
R = 1
$$

:::
:::

::: {.callout-note icon=false collapse="true"}

## 8.2.7

### **Problem:**

Find the first four nonzero coefficients of the Taylor series expansion for the function

$$
f(t) = \frac{1}{1 + t^4}
$$

about $a = 0$. In addition, state the radius of convergence of the series expansion.

### **Solution:**

#### **Rewrite the Function**

The function is expressed as:

$$
f(t) = \frac{1}{1 + t^4}
$$

This can be rewritten in a form suitable for a geometric series expansion:

$$
f(t) = \frac{1}{1 - (-t^4)}
$$

The known power series expansion for $\frac{1}{1 - x}$ is:

$$
\frac{1}{1 - x} = \sum_{n=0}^\infty x^n, \quad \text{for } |x| < 1
$$

Substituting $x = -t^4$, the series becomes:

$$
f(t) = \sum_{n=0}^\infty (-t^4)^n
$$

#### **General Formula for the Terms**

The general term of the series is:

$$
a_n = (-1)^n t^{4n}
$$

#### **Compute the First Four Nonzero Terms**

1. **For $n = 0$:**

$$
a_0 = (-1)^0 t^{4 \cdot 0} = 1
$$

The first term is:

$$
a_0 = 1
$$

2. **For $n = 1$:**

$$
a_1 = (-1)^1 t^{4 \cdot 1} = -t^4
$$

The second term is:

$$
a_1 = -t^4
$$

3. **For $n = 2$:**

$$
a_2 = (-1)^2 t^{4 \cdot 2} = t^8
$$

The third term is:

$$
a_2 = t^8
$$

4. **For $n = 3$:**

$$
a_3 = (-1)^3 t^{4 \cdot 3} = -t^{12}
$$

The fourth term is:

$$
a_3 = -t^{12}
$$

#### **The Taylor Series**

The first four nonzero terms of the Taylor series expansion are:

$$
f(t) = 1 - t^4 + t^8 - t^{12} + \cdots
$$

#### **Radius of Convergence**

The geometric series $\frac{1}{1 - x}$ converges for $|x| < 1$. Substituting $x = -t^4$, the series converges for:

$$
|-t^4| < 1 \quad \implies \quad |t^4| < 1 \quad \implies \quad |t| < 1
$$

Thus, the radius of convergence is:

$$
R = 1
$$

::: {.callout-tip icon=false}

## **Final Answer:**

**First Four Nonzero Terms:**

$$
f(t) = 1 - t^4 + t^8 - t^{12}
$$

**Radius of Convergence:**

$$
R = 1
$$

:::
:::

::: {.callout-note icon=false collapse="true"}

## 8.2.18

### **Problem:**

Find the first four nonzero coefficients of the Taylor series expansion for the integral:

$$
\int_0^t \frac{1}{1 + s^4} \, ds
$$

by first expanding the integrand into its Taylor series and then integrating term by term.

### **Solution:**

#### **Expand the Integrand**

The given integrand is:

$$
\frac{1}{1 + s^4}
$$

Using the result from the previous problem, the Taylor series expansion for $\frac{1}{1 + s^4}$ is:

$$
\frac{1}{1 + s^4} = \sum_{n=0}^\infty (-1)^n s^{4n}
$$

The first several terms of this series are:

$$
\frac{1}{1 + s^4} = 1 - s^4 + s^8 - s^{12} + \cdots
$$

#### **Integrate Term by Term**

The integral is:

$$
\int_0^t \frac{1}{1 + s^4} \, ds = \int_0^t \left(1 - s^4 + s^8 - s^{12} + \cdots \right) \, ds
$$

Integrating each term of the series:

1. **First term:**

$$
\int_0^t 1 \, ds = t
$$

2. **Second term:**

$$
\int_0^t -s^4 \, ds = -\frac{s^5}{5} \bigg|_0^t = -\frac{t^5}{5}
$$

3. **Third term:**

$$
\int_0^t s^8 \, ds = \frac{s^9}{9} \bigg|_0^t = \frac{t^9}{9}
$$

4. **Fourth term:**

$$
\int_0^t -s^{12} \, ds = -\frac{s^{13}}{13} \bigg|_0^t = -\frac{t^{13}}{13}
$$

#### **Combine the Results**

The first four nonzero terms of the Taylor series expansion for the integral are:

$$
\int_0^t \frac{1}{1 + s^4} \, ds = t - \frac{t^5}{5} + \frac{t^9}{9} - \frac{t^{13}}{13} + \cdots
$$

::: {.callout-tip icon=false}

## **Final Answer:**

The Taylor series expansion for the integral is:

$$
\int_0^t \frac{1}{1 + s^4} \, ds = t - \frac{t^5}{5} + \frac{t^9}{9} - \frac{t^{13}}{13} + \cdots
$$

:::
:::

::: {.callout-note icon=false collapse="true"}

## 8.2.19

### **Problem:**

Find the first four nonzero coefficients of the Taylor series expansion for the integral:

$$
\int_0^t e^{-s^2} \, ds
$$

by first expanding the integrand into its Taylor series and then integrating term by term.

### **Solution:**

#### **Expand the Integrand**

The given integrand is:

$$
e^{-s^2}
$$

The Taylor series expansion for $e^x$ is:

$$
e^x = \sum_{n=0}^\infty \frac{x^n}{n!}
$$

Substituting $x = -s^2$, the expansion becomes:

$$
e^{-s^2} = \sum_{n=0}^\infty \frac{(-1)^n s^{2n}}{n!}
$$

The first few terms are:

$$
e^{-s^2} = 1 - s^2 + \frac{s^4}{2!} - \frac{s^6}{3!} + \cdots
$$

#### **Integrate Term by Term**

The integral is:

$$
\int_0^t e^{-s^2} \, ds = \int_0^t \left(1 - s^2 + \frac{s^4}{2} - \frac{s^6}{6} + \cdots \right) \, ds
$$

Integrating each term of the series:

1. **First term:**

$$
\int_0^t 1 \, ds = t
$$

2. **Second term:**

$$
\int_0^t -s^2 \, ds = -\frac{s^3}{3} \bigg|_0^t = -\frac{t^3}{3}
$$

3. **Third term:**

$$
\int_0^t \frac{s^4}{2} \, ds = \frac{1}{2} \cdot \frac{s^5}{5} \bigg|_0^t = \frac{t^5}{10}
$$

4. **Fourth term:**

$$
\int_0^t -\frac{s^6}{6} \, ds = -\frac{1}{6} \cdot \frac{s^7}{7} \bigg|_0^t = -\frac{t^7}{42}
$$

#### **Combine the Results**

The first four nonzero terms of the Taylor series expansion for the integral are:

$$
\int_0^t e^{-s^2} \, ds = t - \frac{t^3}{3} + \frac{t^5}{10} - \frac{t^7}{42} + \cdots
$$

::: {.callout-tip icon=false}

## **Final Answer:**

The Taylor series expansion for the integral is:

$$
\int_0^t e^{-s^2} \, ds = t - \frac{t^3}{3} + \frac{t^5}{10} - \frac{t^7}{42} + \cdots
$$

:::
:::
