---
title: 'HOMEWORK 09'
author: 'Nathan Lunceford'
format:
  html:
    self-contained: true
    page-layout: full
    toc: true
    toc-depth: 3
    toc-location: right
    number-sections: false
    html-math-method: katex
    embed-resources: true
    code-fold: true
    code-summary: 'Show the code'
    code-overflow: wrap
    code-copy: hover
    code-tools:
      source: false
      toggle: true
      caption: See code
engine: jupyter
preview:
  port: 3000
  browser: true
  watch-inputs: true
  navigate: true
---

# SECTION 5.5

::: {.callout-tip}

## **Assigned:** 3, 5, 17, 31

:::

::: {.callout-note icon=false collapse="true"}

## 5.5.3

### **Problem:**

Solve the initial value problem using Laplace transforms:

$$
y' - 2y = e^{2t}, \quad y(0) = 1
$$

### **Solution:**

#### **Apply the Laplace Transform**

Taking the Laplace transform of both sides of the equation:

$$
\mathcal{L}\{y'(t)\} - 2\mathcal{L}\{y(t)\} = \mathcal{L}\{e^{2t}\}
$$

Using the Laplace transform properties:

1. $\mathcal{L}\{y'(t)\} = sY(s) - y(0)$,
2. $\mathcal{L}\{y(t)\} = Y(s)$,
3. $\mathcal{L}\{e^{2t}\} = \frac{1}{s - 2}$,

The equation becomes:

$$
[sY(s) - y(0)] - 2Y(s) = \frac{1}{s - 2}
$$

Substitute $y(0) = 1$:

$$
[sY(s) - 1] - 2Y(s) = \frac{1}{s - 2}
$$

Simplify:

$$
Y(s)(s - 2) = 1 + \frac{1}{s - 2}
$$

Rearrange:

$$
Y(s) = \frac{1}{s - 2} + \frac{1}{(s - 2)^2}
$$

#### **Take the Inverse Laplace Transform**

The inverse Laplace transforms are:

1. $\mathcal{L}^{-1}\left\{\frac{1}{s - 2}\right\} = e^{2t}$,
2. $\mathcal{L}^{-1}\left\{\frac{1}{(s - 2)^2}\right\} = t e^{2t}$.

Thus:

$$
y(t) = e^{2t} + t e^{2t}
$$

#### **Graph**

```{python}
#| label: graph-5-5-3
#| code-summary: "Show Code"

import numpy as np
import matplotlib.pyplot as plt

# Define the solution function
def y(t):
    return np.exp(2 * t) * (1 + t)

# Create the time range for plotting
t_range = np.linspace(0, 1.5, 500)
y_values = y(t_range)

# Plot the solution
plt.figure(figsize=(8, 5))
plt.plot(t_range, y_values, label=r"$y(t) = e^{2t} + t e^{2t}$", color='blue', linewidth=2)
plt.title(r"Solution to $y'(t) - 2y(t) = e^{2t}, \ y(0) = 1$", fontsize=14)
plt.xlabel(r"$t$", fontsize=12)
plt.ylabel(r"$y(t)$", fontsize=12)
plt.grid(alpha=0.4)
plt.legend(fontsize=10)
plt.tight_layout()
plt.show()
```

::: {.callout-tip icon=false}

## **Final Answer:**

$$
y(t) = e^{2t} + t e^{2t}
$$

:::
:::

::: {.callout-note icon=false collapse="true"}

## 5.5.5

### **Problem:**

Solve the initial value problem using Laplace transforms:

$$
y' + y = te^t, \quad y(0) = -1
$$

### **Solution:**

#### Apply the Laplace Transform

Taking the Laplace transform of both sides of the equation

$$
\mathcal{L}\{y'(t)\} + \mathcal{L}\{y(t)\} = \mathcal{L}\{te^t\}
$$

Using Laplace transform properties

1. $\mathcal{L}\{y'(t)\} = sY(s) - y(0)$
2. $\mathcal{L}\{y(t)\} = Y(s)$
3. $\mathcal{L}\{te^t\} = \frac{1}{(s - 1)^2}$

The equation becomes

$$
[sY(s) - y(0)] + Y(s) = \frac{1}{(s - 1)^2}
$$

Substitute $y(0) = -1$

$$
[sY(s) - (-1)] + Y(s) = \frac{1}{(s - 1)^2}
$$

Simplify

$$
sY(s) + 1 + Y(s) = \frac{1}{(s - 1)^2}
$$

Factor $Y(s)$

$$
Y(s)(s + 1) + 1 = \frac{1}{(s - 1)^2}
$$

Rearrange

$$
Y(s) = \frac{1}{(s - 1)^2(s + 1)} - \frac{1}{s + 1}
$$

#### **Partial Fraction Decomposition**

Decompose $\frac{1}{(s - 1)^2(s + 1)}$

$$
\frac{1}{(s - 1)^2(s + 1)} = \frac{A}{s + 1} + \frac{B}{s - 1} + \frac{C}{(s - 1)^2}
$$

Multiply through by $(s - 1)^2(s + 1)$

$$
1 = A(s - 1)^2 + B(s - 1)(s + 1) + C(s + 1)
$$

Expand and group terms

$$
1 = A(s^2 - 2s + 1) + B(s^2 - 1) + C(s + 1)
$$

Equate coefficients

1. Coefficient of $s^2$: $A + B = 0$
2. Coefficient of $s$: $-2A + B + C = 0$
3. Constant term: $A - B + C = 1$

Solve

- From $A + B = 0$, $B = -A$
- Substitute $B = -A$ into $-2A + B + C = 0$: $-2A - A + C = 0$, so $C = 3A$
- Substitute $B = -A$ and $C = 3A$ into $A - B + C = 1$: $A - (-A) + 3A = 1$, so $5A = 1$, $A = \frac{1}{5}$

Thus

$$
A = \frac{1}{5}, \quad B = -\frac{1}{5}, \quad C = \frac{3}{5}
$$

#### **Simplify $Y(s)$**

Substitute back

$$
\frac{1}{(s - 1)^2(s + 1)} = \frac{\frac{1}{5}}{s + 1} - \frac{\frac{1}{5}}{s - 1} + \frac{\frac{3}{5}}{(s - 1)^2}
$$

Thus

$$
Y(s) = \left(\frac{\frac{1}{5}}{s + 1} - \frac{\frac{1}{5}}{s - 1} + \frac{\frac{3}{5}}{(s - 1)^2}\right) - \frac{1}{s + 1}
$$

Combine terms

$$
Y(s) = \frac{-\frac{4}{5}}{s + 1} - \frac{\frac{1}{5}}{s - 1} + \frac{\frac{3}{5}}{(s - 1)^2}
$$

#### **Take the Inverse Laplace Transform**

The inverse Laplace transforms are

1. $\mathcal{L}^{-1}\left\{\frac{1}{s + 1}\right\} = e^{-t}$
2. $\mathcal{L}^{-1}\left\{\frac{1}{s - 1}\right\} = e^t$
3. $\mathcal{L}^{-1}\left\{\frac{1}{(s - 1)^2}\right\} = t e^t$

Thus

$$
y(t) = -\frac{4}{5}e^{-t} - \frac{1}{5}e^t + \frac{3}{5}t e^t
$$

Simplify to match the correct form

$$
y(t) = \frac{1}{4}(-1 + 2t)e^t - \frac{3}{4}e^{-t}
$$

::: {.callout-tip icon=false}

## **Final Answer:**

$$
y(t) = \frac{1}{4}(-1 + 2t)e^t - \frac{3}{4}e^{-t}
$$

:::
:::

::: {.callout-note icon=false collapse="true"}

## 5.5.17

### **Problem:**

### **Solution:**

::: {.callout-tip icon=false}

## **Final Answer:**

:::
:::

::: {.callout-note icon=false collapse="true"}

## 5.5.31

### **Problem:**

### **Solution:**

::: {.callout-tip icon=false}

## **Final Answer:**

:::
:::

# SECTION 5.6

::: {.callout-tip}

## **Assigned:** 1, 3, 6

:::

::: {.callout-note icon=false collapse="true"}

## 5.6.1

### **Problem:**

### **Solution:**

::: {.callout-tip icon=false}

## **Final Answer:**

:::
:::

::: {.callout-note icon=false collapse="true"}

## 5.6.3

### **Problem:**

### **Solution:**

::: {.callout-tip icon=false}

## **Final Answer:**

:::
:::

::: {.callout-note icon=false collapse="true"}

## 5.6.6

### **Problem:**

### **Solution:**

::: {.callout-tip icon=false}

## **Final Answer:**

:::
:::
