---
title: 'HOMEWORK 06'
author: 'Nathan Lunceford'
format:
  html:
    self-contained: true
    page-layout: full
    toc: true
    toc-depth: 2
    toc-location: right
    number-sections: false
    html-math-method: katex
    code-fold: true
    code-summary: 'Show the code'
    code-overflow: wrap
    code-copy: hover
    code-tools:
      source: false
      toggle: true
      caption: See code
editor:
  render-on-save: true
---

# SECTION 4.5

::: {.callout-tip}

## **Assigned:** 1, 3

:::

::: {.callout-note icon=false collapse="true"}

## 4.5.1

### **Problem:**

For the given initial-value problem $y(0) = y'(0) = 0$, solve for $y(t)$ in an
undamped spring-mass system with the specified parameters. Additionally,
determine the maximum displacement of the mass, state if beats or resonance are
present, and sketch the solution.

Given parameters:

- $m = 1$
- $k = 25$
- $f(t) = 0.01 \cos(5t)$

### **Solution:**

#### Solve the Homogeneous Equation

The corresponding homogeneous equation is:

$$
y_h'' + 25y_h = 0
$$

The characteristic equation is:

$$
r^2 + 25 = 0 \quad \Rightarrow \quad r = \pm 5i
$$

The general solution to the homogeneous equation is:

$$
y_h(t) = C_1 \cos(5t) + C_2 \sin(5t)
$$

#### Find the Particular Solution

The non-homogeneous term is $f(t) = \frac{1}{100} \cos(5t)$. Since this term has
the same frequency as the homogeneous solution, **resonance** occurs.

To account for resonance, assume a particular solution of the form:

$$
y_p(t) = t \left( A \cos(5t) + B \sin(5t) \right)
$$

#### Compute the Derivatives of $y_p(t)$

1. **First Derivative $y_p'(t)$:**

   Using the product rule:

   $$
   \begin{aligned}
   y_p'(t) &= A \cos(5t) + B \sin(5t) + t \left( -5A \sin(5t) + 5B \cos(5t) \right) \\
   &= A \cos(5t) + B \sin(5t) - 5A t \sin(5t) + 5B t \cos(5t)
   \end{aligned}
   $$

2. **Second Derivative $y_p''(t)$:**

   Differentiating $y_p'(t)$:

   $$
   \begin{aligned}
   y_p''(t) &= -5A \sin(5t) + 5B \cos(5t) - 5A \sin(5t) + 5B \cos(5t) \\
   &\quad - 25A t \cos(5t) - 25B t \sin(5t) \\
   &= -10A \sin(5t) + 10B \cos(5t) - 25A t \cos(5t) - 25B t \sin(5t)
   \end{aligned}
   $$

#### Substitute into the Original Equation

$$
y_p''(t) + 25 y_p(t) = \frac{1}{100} \cos(5t)
$$

Plugging in the expressions:

$$
\begin{aligned}
&\left[ -10A \sin(5t) + 10B \cos(5t) - 25A t \cos(5t) - 25B t \sin(5t) \right] \\
&\quad + 25 \left[ A t \cos(5t) + B t \sin(5t) \right] = \frac{1}{100} \cos(5t)
\end{aligned}
$$

Simplifying:

$$
-10A \sin(5t) + 10B \cos(5t) = \frac{1}{100} \cos(5t)
$$

#### Equate Coefficients and Solve for $A$ and $B$

1. Coefficient of $\sin(5t)$:

   $$
   -10A = 0 \quad \Rightarrow \quad A = 0
   $$

2. Coefficient of $\cos(5t)$:

   $$
   10B = \frac{1}{100} \quad \Rightarrow \quad B = \frac{1}{1000}
   $$

#### Particular Solution

Substitute $A = 0$ and $B = \frac{1}{1000}$:

$$
y_p(t) = t \left( 0 \cdot \cos(5t) + \frac{1}{1000} \sin(5t) \right) = \frac{t}{1000} \sin(5t)
$$

#### General Solution

$$
y(t) = y_h(t) + y_p(t) = C_1 \cos(5t) + C_2 \sin(5t) + \frac{t}{1000} \sin(5t)
$$

#### Apply Initial Conditions

Given $y(0) = 0$ and $y'(0) = 0$:

1. **At $t = 0$:**

   $$
   y(0) = C_1 \cos(0) + C_2 \sin(0) + \frac{0}{1000} \sin(0) = C_1
   $$

   Since $y(0) = 0$:

   $$
   C_1 = 0
   $$

2. **First Derivative $y'(t)$:**

   $$
   \begin{aligned}
   y'(t) &= -5 C_1 \sin(5t) + 5 C_2 \cos(5t) + \frac{d}{dt} \left( \frac{t}{1000} \sin(5t) \right) \\
   &= 5 C_2 \cos(5t) + \frac{1}{1000} \sin(5t) + \frac{5t}{1000} \cos(5t)
   \end{aligned}
   $$

   **At $t = 0$:**

   $$
   y'(0) = 5 C_2 \cos(0) + \frac{1}{1000} \sin(0) + \frac{5 \cdot 0}{1000} \cos(0) = 5 C_2
   $$

   Since $y'(0) = 0$:

   $$
   C_2 = 0
   $$

#### Solution

With $C_1 = 0$ and $C_2 = 0$, the solution simplifies to:

$$
y(t) = \frac{t}{1000} \sin(5t) = \frac{t}{10^3} \sin(5t)
$$

#### Maximum Displacement

Since resonance occurs, the amplitude of $y(t) = \frac{t}{1000} \sin(5t)$ grows
without bound as $t \to \infty$. So the maximum displacement increases
indefinitely over time due to resonance.

#### Presence of Beats or Resonance

Resonance is present because the forcing frequency matches the natural frequency
of the system.

#### Graph

```{python}
#| label: graph-4-5-1
#| code-summary: "Show Code"

import numpy as np
import matplotlib.pyplot as plt

t = np.linspace(0, 50, 1000)

y = (t / 1000) * np.sin(5 * t)

plt.figure(figsize=(10, 6))
plt.plot(t, y, label=r"$y(t) = \frac{t}{1000} \sin(5t)$")
plt.xlabel("Time (t)")
plt.ylabel("Displacement (y)")
plt.title("Graph of Solution")
plt.legend()
plt.grid(True)
plt.show()

```

::: {.callout-tip icon=false}

## **Final Answer:**

$$
y(t) = \frac{t}{1000} \sin(5t)
$$

The system exhibits resonance, leading to an unbounded increase in displacement
over time.

:::
:::

::: {.callout-note icon=false collapse="true"}

## 4.5.3

### **Problem:**

In the given initial-value problem, solve for $y(t)$ in an undamped spring-mass
system with the specified parameters. Additionally, determine the maximum
displacement of the mass, state if beats or resonance are present, and sketch
the solution.

Given parameters:

- $m = 1$
- $k = 36$
- $f(t) = 2 e^{6t}$
- Initial conditions: $y(0) = 0$ and $y'(0) = 0$

### **Solution:**

#### Solve the Homogeneous Equation

The homogeneous equation is:

$$
y_h'' + 36 y_h = 0
$$

The characteristic equation is:

$$
r^2 + 36 = 0 \quad \Rightarrow \quad r = \pm 6i
$$

The general solution to the homogeneous equation is:

$$
y_h(t) = C_1 \cos(6t) + C_2 \sin(6t)
$$

#### Find the Particular Solution

The non-homogeneous term is $f(t) = 2 e^{6t}$. Since this is an exponential
function and does not overlap with the homogeneous solution, assume a particular
solution of the form:

$$
y_p(t) = A e^{6t}
$$

#### Compute the Derivatives of $y_p(t)$

1. **First Derivative $y_p'(t)$:**

   $$
   y_p'(t) = 6 A e^{6t}
   $$

2. **Second Derivative $y_p''(t)$:**

   $$
   y_p''(t) = 36 A e^{6t}
   $$

#### Substitute into the Original Equation

Substitute $y_p(t)$, $y_p'(t)$, and $y_p''(t)$ into the differential equation:

$$
y_p'' + 36 y_p = 2 e^{6t}
$$

Substitute the expressions:

$$
36 A e^{6t} + 36 A e^{6t} = 2 e^{6t}
$$

Simplify:

$$
72 A e^{6t} = 2 e^{6t}
$$

Divide both sides by $e^{6t}$:

$$
72 A = 2
$$

#### Solve for $A$

$$
A = \frac{2}{72} = \frac{1}{36}
$$

#### Particular Solution

$$
y_p(t) = \frac{1}{36} e^{6t}
$$

#### General Solution

$$
y(t) = y_h(t) + y_p(t) = C_1 \cos(6t) + C_2 \sin(6t) + \frac{1}{36} e^{6t}
$$

#### Apply Initial Conditions

Given $y(0) = 0$ and $y'(0) = 0$, we can solve for $C_1$ and $C_2$.

1. **At $t = 0$:**

   $$
   y(0) = C_1 \cos(0) + C_2 \sin(0) + \frac{1}{36} e^{0} = C_1 + \frac{1}{36}
   $$

   Since $y(0) = 0$:

   $$
   C_1 + \frac{1}{36} = 0 \quad \Rightarrow \quad C_1 = -\frac{1}{36}
   $$

2. **First Derivative $y'(t)$:**

   Calculate $y'(t)$:

   $$
   y'(t) = -6 C_1 \sin(6t) + 6 C_2 \cos(6t) + \frac{1}{36} \cdot 6 e^{6t} = -6 C_1 \sin(6t) + 6 C_2 \cos(6t) + \frac{1}{6} e^{6t}
   $$

   At $t = 0$:

   $$
   y'(0) = -6 C_1 \sin(0) + 6 C_2 \cos(0) + \frac{1}{6} e^{0} = 6 C_2 + \frac{1}{6}
   $$

   Since $y'(0) = 0$:

   $$
   6 C_2 + \frac{1}{6} = 0 \quad \Rightarrow \quad C_2 = -\frac{1}{36}
   $$

#### Solution

Substitute $C_1 = -\frac{1}{36}$ and $C_2 = -\frac{1}{36}$:

$$
y(t) = -\frac{1}{36} \cos(6t) - \frac{1}{36} \sin(6t) + \frac{1}{36} e^{6t}
$$

#### Determine Maximum Displacement

The term $\frac{1}{36} e^{6t}$ grows exponentially as $t \to \infty$, leading to
an unbounded increase in displacement. Therefore, the maximum displacement
increases without bound over time.

#### Presence of Beats or Resonance

- **Resonance is not present** in this system, as the forcing frequency does not
  match the natural frequency.
- **Beats are not present** since there are no two competing frequencies close
  to each other.

#### Graph

```{python}
#| label: graph-4-5-3
#| code-summary: "Show Code"

t = np.linspace(0, 2, 1000)

y = (-1/36) * np.cos(6 * t) - (1/36) * np.sin(6 * t) + (1/36) * np.exp(6 * t)

plt.figure(figsize=(10, 6))
plt.plot(t, y, label=r"$y(t) = -\frac{1}{36} \cos(6t) - \frac{1}{36} \sin(6t) + \frac{1}{36} e^{6t}$")
plt.xlabel("Time (t)")
plt.ylabel("Displacement (y)")
plt.title("Graph of Solution Showing Exponential Growth in Displacement")
plt.legend()
plt.grid(True)
plt.show()
```

::: {.callout-tip icon=false}

## **Final Answer:**

$$
y(t) = -\frac{1}{36} \cos(6t) - \frac{1}{36} \sin(6t) + \frac{1}{36} e^{6t}
$$

- The system does not exhibit resonance or beats.
- The maximum displacement grows exponentially due to the $\frac{1}{36} e^{6t}$
  term.

:::
:::

# SECTION 3.2

::: {.callout-tip}

## **Assigned:** 9, 11, 17

:::

::: {.callout-note icon=false collapse="true"}

## 3.2.9

### **Problem:**

Consider the system of differential equations given by

$$
x_1' = -x_1 + 2x_2
$$

$$
x_2' = -7x_1 + 8x_2
$$

(a) Determine a matrix $\mathbf{A}$ so that the system may be written in the
form $\mathbf{x}' = \mathbf{A} \mathbf{x}$.

(b) Determine all constant solutions to $\mathbf{x}' = \mathbf{A} \mathbf{x}$.

(c) Compute the eigenvalues and eigenvectors of $\mathbf{A}$.

(d) Determine all straight-line solutions to
$\mathbf{x}' = \mathbf{A} \mathbf{x}$.

(e) Find a more general solution to $\mathbf{x}' = \mathbf{A} \mathbf{x}$ by
taking all possible linear combinations of the straight-line solutions from (d).

(f) Solve the initial-value problem $\mathbf{x}' = \mathbf{A} \mathbf{x}$,
$\mathbf{x}(0) = \begin{bmatrix} -2 \\ 0 \end{bmatrix}$. Discuss the graphical
behavior of this solution.

### **Solution:**

#### (a) Determine the Matrix $\mathbf{A}$

The system is:

$$
x_1' = -x_1 + 2x_2
$$

$$
x_2' = -7x_1 + 8x_2
$$

This can be written in matrix form as:

$$
\mathbf{x}' = \begin{bmatrix} -1 & 2 \\ -7 & 8 \end{bmatrix} \mathbf{x}
$$

So, the matrix $\mathbf{A}$ is:

$$
\mathbf{A} = \begin{bmatrix} -1 & 2 \\ -7 & 8 \end{bmatrix}
$$

#### (b) Determine All Constant Solutions

Constant solutions satisfy $\mathbf{x}' = \mathbf{0}$, so:

$$
\mathbf{A} \mathbf{x} = \mathbf{0}
$$

This leads to the homogeneous system:

$$
- x_1 + 2 x_2 = 0
$$

$$
-7 x_1 + 8 x_2 = 0
$$

Solving, we find that $x_1 = x_2 = 0$. So, the only constant solution is:

$$
\mathbf{x} = \begin{bmatrix} 0 \\ 0 \end{bmatrix}
$$

#### (c) Compute the Eigenvalues and Eigenvectors of $\mathbf{A}$

Compute the characteristic equation:

$$
\det(\mathbf{A} - \lambda \mathbf{I}) = 0
$$

$$
\begin{vmatrix} -1 - \lambda & 2 \\ -7 & 8 - \lambda \end{vmatrix} = (-1 - \lambda)(8 - \lambda) - (-7)(2) = 0
$$

Simplify:

$$
\lambda^2 - 7\lambda + 6 = 0 \implies (\lambda - 6)(\lambda - 1) = 0
$$

Eigenvalues are $\lambda_1 = 6$ and $\lambda_2 = 1$.

For $\lambda = 1$:

$$
(\mathbf{A} - \mathbf{I})\mathbf{v} = \mathbf{0} \implies \begin{bmatrix} -2 & 2 \\ -7 & 7 \end{bmatrix} \mathbf{v} = \mathbf{0}
$$

This yields $v_1 = v_2$. So, an eigenvector is:

$$
\mathbf{v}_1 = \begin{bmatrix} 1 \\ 1 \end{bmatrix}
$$

For $\lambda = 6$:

$$
(\mathbf{A} - 6\mathbf{I})\mathbf{v} = \mathbf{0} \implies \begin{bmatrix} -7 & 2 \\ -7 & 2 \end{bmatrix} \mathbf{v} = \mathbf{0}
$$

This gives $v_2 = \frac{7}{2}v_1$. An eigenvector is:

$$
\mathbf{v}_2 = \begin{bmatrix} 2 \\ 7 \end{bmatrix}
$$

#### (d) Determine All Straight-Line Solutions

Straight-line solutions are of the form
$\mathbf{x}(t) = \mathbf{v} e^{\lambda t}$:

$$
\mathbf{x}_1(t) = c_1 \begin{bmatrix} 1 \\ 1 \end{bmatrix} e^{t}, \quad \mathbf{x}_2(t) = c_2 \begin{bmatrix} 2 \\ 7 \end{bmatrix} e^{6t}
$$

#### (e) General Solution as a Linear Combination of Straight-Line Solutions

$$
\mathbf{x}(t) = c_1 \begin{bmatrix} 1 \\ 1 \end{bmatrix} e^{t} + c_2 \begin{bmatrix} 2 \\ 7 \end{bmatrix} e^{6t}
$$

#### (f) Solve the Initial-Value Problem

Initial condition $\mathbf{x}(0) = \begin{bmatrix} -2 \\ 0 \end{bmatrix}$:

$$
\begin{cases}
c_1 + 2c_2 = -2 \\
c_1 + 7c_2 = 0
\end{cases}
$$

Solving:

$$
c_2 = \frac{2}{5}, \quad c_1 = -\frac{14}{5}
$$

So the solution is:

$$
\mathbf{x}(t) = -\frac{14}{5} \begin{bmatrix} 1 \\ 1 \end{bmatrix} e^{t} + \frac{2}{5} \begin{bmatrix} 2 \\ 7 \end{bmatrix} e^{6t}
$$

#### Graphical Behavior of the Solution

- As $t \to \infty$, $e^{6t}$ dominates $e^{t}$, so $\mathbf{x}(t)$ grows
  exponentially in the direction of $\begin{bmatrix} 2 \\ 7 \end{bmatrix}$.

::: {.callout-tip icon=false}

## **Final Answer:**

**(a)** An explicit matrix $\mathbf{A}$ is

$$
\mathbf{A} = \begin{bmatrix} -1 & 2 \\ -7 & 8 \end{bmatrix}
$$

**(b)** All constant solutions satisfy

$$
\mathbf{x} = \begin{bmatrix} 0 \\ 0 \end{bmatrix}
$$

**(c)** Eigenvalues are $\lambda = 6$ and $\lambda = 1$; corresponding
eigenvectors are

$$
\mathbf{v}_1 = \begin{bmatrix} 1 \\ 1 \end{bmatrix},\quad \mathbf{v}_2 = \begin{bmatrix} 2 \\ 7 \end{bmatrix}
$$

**(d)** All straight-line solutions are

$$
\mathbf{x}(t) = c_1 \begin{bmatrix} 1 \\ 1 \end{bmatrix} e^{t} + c_2 \begin{bmatrix} 2 \\ 7 \end{bmatrix} e^{6t}
$$

**(e)** The general solution is the linear combination of straight-line
solutions:

$$
\mathbf{x}(t) = c_1 \begin{bmatrix} 1 \\ 1 \end{bmatrix} e^{t} + c_2 \begin{bmatrix} 2 \\ 7 \end{bmatrix} e^{6t}
$$

**(f)** Solving the initial-value problem gives:

$$
\mathbf{x}(t) = -\frac{14}{5} \begin{bmatrix} 1 \\ 1 \end{bmatrix} e^{t} + \frac{2}{5} \begin{bmatrix} 2 \\ 7 \end{bmatrix} e^{6t}
$$

**Graphical behavior:** As $t \to \infty$, $e^{6t}$ dominates $e^{t}$, so
$\mathbf{x}(t)$ grows exponentially in the direction of
$\begin{bmatrix} 2 \\ 7 \end{bmatrix}$.

:::
:::

::: {.callout-note icon=false collapse="true"}

## 3.2.11

### **Problem:**

Consider the system of differential equations given by

$$
x_1' = -2x_1 + x_2
$$

$$
x_2' = -2x_2
$$

(a) Determine a matrix $\mathbf{A}$ so that the system may be written in the
form $\mathbf{x}' = \mathbf{A} \mathbf{x}$.

(b) Determine all constant solutions to $\mathbf{x}' = \mathbf{A} \mathbf{x}$.

(c) Compute the eigenvalues and eigenvectors of $\mathbf{A}$.

(d) Determine all straight-line solutions to
$\mathbf{x}' = \mathbf{A} \mathbf{x}$.

(e) Find a more general solution to $\mathbf{x}' = \mathbf{A} \mathbf{x}$ by
taking all possible linear combinations of the straight-line solutions from (d).

(f) Attempt to solve the initial-value problem
$\mathbf{x}' = \mathbf{A} \mathbf{x}$,
$\mathbf{x}(0) = \begin{bmatrix} 1 \\ 1 \end{bmatrix}$. What does this tell you
about the proposed general solution in (e)?

### **Solution:**

#### (a) Determine the Matrix $\mathbf{A}$

The system is:

$$
x_1' = -2x_1 + x_2
$$

$$
x_2' = -2x_2
$$

This can be written in matrix form as:

$$
\mathbf{x}' = \begin{bmatrix} -2 & 1 \\ 0 & -2 \end{bmatrix} \mathbf{x}
$$

So, the matrix $\mathbf{A}$ is:

$$
\mathbf{A} = \begin{bmatrix} -2 & 1 \\ 0 & -2 \end{bmatrix}
$$

#### (b) Determine All Constant Solutions

Constant solutions satisfy $\mathbf{x}' = \mathbf{0}$, so:

$$
\mathbf{A} \mathbf{x} = \mathbf{0}
$$

This leads to the homogeneous system:

$$
-2 x_1 + x_2 = 0
$$

$$
-2 x_2 = 0
$$

From the second equation, $x_2 = 0$. Substituting into the first equation gives
$x_1 = 0$. Therefore, the only constant solution is:

$$
\mathbf{x} = \begin{bmatrix} 0 \\ 0 \end{bmatrix}
$$

#### (c) Compute the Eigenvalues and Eigenvectors of $\mathbf{A}$

Compute the characteristic equation:

$$
\det(\mathbf{A} - \lambda \mathbf{I}) = 0
$$

$$
\begin{vmatrix} -2 - \lambda & 1 \\ 0 & -2 - \lambda \end{vmatrix} = (-2 - \lambda)^2 = 0
$$

$\lambda = -2$ is a repeated eigenvalue.

To find the eigenvectors, solve
$(\mathbf{A} + 2\mathbf{I}) \mathbf{v} = \mathbf{0}$:

$$
\begin{bmatrix} 0 & 1 \\ 0 & 0 \end{bmatrix} \mathbf{v} = \mathbf{0}
$$

This gives $v_2 = 0$, so an eigenvector corresponding to $\lambda = -2$ is:

$$
\mathbf{v}_1 = \begin{bmatrix} 1 \\ 0 \end{bmatrix}
$$

Since $\lambda = -2$ is a repeated eigenvalue with only one linearly independent
eigenvector, find a generalized eigenvector by solving
$(\mathbf{A} + 2\mathbf{I}) \mathbf{v} = \mathbf{v}_1$:

$$
\begin{bmatrix} 0 & 1 \\ 0 & 0 \end{bmatrix} \mathbf{v} = \begin{bmatrix} 1 \\ 0 \end{bmatrix}
$$

This gives $v_2 = 1$. So a generalized eigenvector is:

$$
\mathbf{v}_2 = \begin{bmatrix} 0 \\ 1 \end{bmatrix}
$$

#### (d) Determine All Straight-Line Solutions

Straight-line solutions are of the form
$\mathbf{x}(t) = \mathbf{v} e^{\lambda t}$. Since there is only one eigenvector,
we have a solution:

$$
\mathbf{x}_1(t) = c_1 \begin{bmatrix} 1 \\ 0 \end{bmatrix} e^{-2t}
$$

#### (e) General Solution Using the Generalized Eigenvector

Since there is a repeated eigenvalue and a generalized eigenvector, the general
solution takes the form:

$$
\mathbf{x}(t) = c_1 \mathbf{v}_1 e^{-2t} + c_2 (\mathbf{v}_2 t e^{-2t} + \mathbf{v}_1 e^{-2t})
$$

Substituting $\mathbf{v}_1 = \begin{bmatrix} 1 \\ 0 \end{bmatrix}$ and
$\mathbf{v}_2 = \begin{bmatrix} 0 \\ 1 \end{bmatrix}$:

$$
\mathbf{x}(t) = c_1 \begin{bmatrix} 1 \\ 0 \end{bmatrix} e^{-2t} + c_2 \left( \begin{bmatrix} 0 \\ 1 \end{bmatrix} t e^{-2t} + \begin{bmatrix} 1 \\ 0 \end{bmatrix} e^{-2t} \right)
$$

Simplifying, the general solution is:

$$
\mathbf{x}(t) = \left( c_1 + c_2 \right) \begin{bmatrix} 1 \\ 0 \end{bmatrix} e^{-2t} + c_2 \begin{bmatrix} 0 \\ t \end{bmatrix} e^{-2t}
$$

#### (f) Solve the Initial-Value Problem

Given $\mathbf{x}(0) = \begin{bmatrix} 1 \\ 1 \end{bmatrix}$, apply the
initial conditions:

$$
\begin{bmatrix} 1 \\ 1 \end{bmatrix} = \left( c_1 + c_2 \right) \begin{bmatrix} 1 \\ 0 \end{bmatrix} + c_2 \begin{bmatrix} 0 \\ 1 \end{bmatrix}
$$

This gives the system:

$$
c_1 + c_2 = 1
$$

$$
c_2 = 1
$$

Solving these, $c_2 = 1$ and $c_1 = 0$. So, the solution to the
initial-value problem is:

$$
\mathbf{x}(t) = \begin{bmatrix} 1 \\ 0 \end{bmatrix} e^{-2t} + \begin{bmatrix} 0 \\ t \end{bmatrix} e^{-2t} = \begin{bmatrix} e^{-2t} \\ t e^{-2t} \end{bmatrix}
$$

#### Interpretation of the Solution

The solution
$\mathbf{x}(t) = \begin{bmatrix} e^{-2t} \\ t e^{-2t} \end{bmatrix}$ shows that
as $t \to \infty$, both components approach zero because of the $e^{-2t}$
factor. However, the term $t e^{-2t}$ causes the solution to decay slower in the
$x_2$-direction, resulting in a solution that initially grows in the
$x_2$-direction before eventually decaying to zero.

::: {.callout-tip icon=false}

## **Final Answer:**

**(a)** An explicit matrix $\mathbf{A}$ is

$$
\mathbf{A} = \begin{bmatrix} -2 & 1 \\ 0 & -2 \end{bmatrix}
$$

**(b)** The only constant solution is

$$
\mathbf{x} = \begin{bmatrix} 0 \\ 0 \end{bmatrix}
$$

**(c)** The eigenvalue is $\lambda = -2$ (repeated); corresponding eigenvectors
are

$$
\mathbf{v}_1 = \begin{bmatrix} 1 \\ 0 \end{bmatrix}
$$

with generalized eigenvector

$$
\mathbf{v}_2 = \begin{bmatrix} 0 \\ 1 \end{bmatrix}
$$

**(d)** A straight-line solution is

$$
\mathbf{x}_1(t) = c_1 \begin{bmatrix} 1 \\ 0 \end{bmatrix} e^{-2t}
$$

**(e)** The general solution is

$$
\mathbf{x}(t) = \left( c_1 + c_2 \right) \begin{bmatrix} 1 \\ 0 \end{bmatrix} e^{-2t} + c_2 \begin{bmatrix} 0 \\ t \end{bmatrix} e^{-2t}
$$

**(f)** The solution to the initial-value problem is

$$
\mathbf{x}(t) = \begin{bmatrix} e^{-2t} \\ t e^{-2t} \end{bmatrix}
$$

**Interpretation:** The term $t e^{-2t}$ results in an initial growth in the
$x_2$-direction before the solution eventually decays to zero, indicating a
slower decay in the $x_2$-component due to the generalized eigenvector.

:::
:::

::: {.callout-note icon=false collapse="true"}

## 3.2.17

### **Problem:**

Convert the second-order differential equation

$$
y'' + y' - 12y = 0
$$

into a system of first-order equations through an appropriate substitution.

### **Solution:**

To convert this into a first-order system, let:

$$
x_1 = y
$$

$$
x_2 = y'
$$

$$
x_1' = y' = x_2
$$

$$
x_2' = y'' = -y' + 12y = -x_2 + 12x_1
$$

The system can be written as:

$$
x_1' = x_2
$$

$$
x_2' = -x_2 + 12x_1
$$

or in matrix form:

$$
\mathbf{x}' = \begin{bmatrix} 0 & 1 \\ 12 & -1 \end{bmatrix} \mathbf{x}
$$

where

$$
\mathbf{x} = \begin{bmatrix} x_1 \\ x_2 \end{bmatrix} = \begin{bmatrix} y \\ y' \end{bmatrix}
$$

::: {.callout-tip icon=false}

## **Final Answer:**

The equivalent system of first-order equations is:

$$
\begin{bmatrix} x_1 \\ x_2 \end{bmatrix}' = \begin{bmatrix} 0 & 1 \\ 12 & -1 \end{bmatrix} \begin{bmatrix} x_1 \\ x_2 \end{bmatrix}
$$

:::
:::

# SECTION 3.3

::: {.callout-tip}

## **Assigned:** 4, 5, 11, 12

:::

# SECTION 3.4

::: {.callout-tip}

## **Assigned:** 1, 3, 7, 13

:::

# SECTION 3.5

::: {.callout-tip}

## **Assigned:** 9, 11, 15, 17

:::
