---
title: "EXAM 03 PRACTICE"
format:
  html:
    self-contained: true
    page-layout: full
    toc: true
    toc-depth: 2
    toc-location: right
    number-sections: false
    html-math-method: katex
    code-fold: true
    code-summary: "Show the code"
    code-overflow: wrap
    code-copy: hover
    code-tools:
        source: false
        toggle: true
        caption: See code
---


## **Spring-Mass Equation Problems**



::: {.callout-tip collapse="true"}
## **Formulas**

The undamped, undriven spring-mass system is represented by:

$$
y'' + \frac{k}{m} y = 0
$$

Where:

- $k$ is the spring constant, indicating the stiffness of the spring.
- $m$ is the mass of the object attached to the spring.
- $y$ is the displacement of the mass from its equilibrium position.

The general solution to this differential equation is:

$$
y_h = c_1 \cos \left( \sqrt{\frac{k}{m}} \, t \right) + c_2 \sin \left( \sqrt{\frac{k}{m}} \, t \right)
$$

Where:

- $y_h$ is the general solution to the homogeneous equation.
- $c_1$ and $c_2$ are constants determined by initial conditions.
- $\sqrt{\frac{k}{m}}$ is the natural angular frequency of the undamped system, often denoted as $\omega = \sqrt{\frac{k}{m}}$.

For a damped, driven spring-mass system, we use:

$$
y'' + \frac{c}{m} y' + \frac{k}{m} y = \frac{1}{m} F(t)
$$

where:

- $m$: Mass of the object.
- $k$: Spring constant, measuring the stiffness of the spring. A higher $k$ indicates a stiffer spring.
- $c$: Damping constant, representing resistance (e.g., due to friction or air resistance) opposing the motion. A higher $c$ implies greater resistance and faster energy dissipation.
- $y(t)$: Displacement of the mass from its equilibrium position at time $t$.
- $F(t)$: External force applied to the system as a function of time.

The terms in the equation represent:

- $y''$: Acceleration of the mass.
- $\frac{c}{m} y'$: Damping term, proportional to the velocity $y'$ and damping constant $c$.
- $\frac{k}{m} y$: Restoring force term, proportional to displacement $y$ and spring constant $k$.
- $\frac{1}{m} F(t)$: External force per unit mass acting on the system.
:::

::: {.callout-note icon=false collapse="true"}
## **Problem**
Consider the initial-value problem for the undamped spring-mass system:

$$
y'' + 25y = 0.01 \cos(5t)
$$

with parameters:

- $m = 1$
- $k = 25$
- $F(t) = 0.01 \cos(5t)$
- Initial conditions: $y(0) = 0$ and $y'(0) = 0$

Solve for $y(t)$, determine the maximum displacement, and state if resonance or beats are present.

:::

::: {.callout-tip icon=false collapse="true"}
## **Solution:**

### Solve the Homogeneous Equation

The corresponding homogeneous equation is:

$$
y_h'' + 25y_h = 0
$$

The characteristic equation is:

$$
r^2 + 25 = 0 \quad \Rightarrow \quad r = \pm 5i
$$

The general solution to the homogeneous equation is:

$$
y_h(t) = C_1 \cos(5t) + C_2 \sin(5t)
$$

### Find the Particular Solution

The non-homogeneous term is $f(t) = \dfrac{1}{100} \cos(5t)$. Since this term has the same frequency as the homogeneous solution, **resonance** occurs.

To account for resonance, assume a particular solution of the form:

$$
y_p(t) = t \left( A \cos(5t) + B \sin(5t) \right)
$$

### Compute the Derivatives of $y_p(t)$

1. **First Derivative $y_p'(t)$:**

Using the product rule:

$$
\begin{aligned}
y_p'(t) &= A \cos(5t) + B \sin(5t) + t \left( -5A \sin(5t) + 5B \cos(5t) \right) \\
&= A \cos(5t) + B \sin(5t) - 5A t \sin(5t) + 5B t \cos(5t)
\end{aligned}
$$

2. **Second Derivative $y_p''(t)$:**

Differentiating $y_p'(t)$:

$$
\begin{aligned}
y_p''(t) &= -5A \sin(5t) + 5B \cos(5t) - 5A \sin(5t) + 5B \cos(5t) \\
&\quad - 5A t \cos(5t) - 5B t \sin(5t) \cdot 5 \\
&= -10A \sin(5t) + 10B \cos(5t) - 25A t \cos(5t) - 25B t \sin(5t)
\end{aligned}
$$

### Substitute into the Original Equation

Substitute $y_p(t)$ and its derivatives into the original equation:

$$
y_p''(t) + 25 y_p(t) = \dfrac{1}{100} \cos(5t)
$$

Plug in the expressions:

$$
\begin{aligned}
&\left[ -10A \sin(5t) + 10B \cos(5t) - 25A t \cos(5t) - 25B t \sin(5t) \right] \\
&\quad + 25 \left[ t A \cos(5t) + t B \sin(5t) \right] = \dfrac{1}{100} \cos(5t)
\end{aligned}
$$

Simplify:

$$
-10A \sin(5t) + 10B \cos(5t) = \dfrac{1}{100} \cos(5t)
$$

### Equate Coefficients and Solve for $A$ and $B$

Set up the equations by equating the coefficients of $\sin(5t)$ and $\cos(5t)$:

1. Coefficient of $\sin(5t)$:

   $$
   -10A = 0 \quad \Rightarrow \quad A = 0
   $$

2. Coefficient of $\cos(5t)$:

   $$
   10B = \dfrac{1}{100} \quad \Rightarrow \quad B = \dfrac{1}{100} \times \dfrac{1}{10} = \dfrac{1}{1000}
   $$

### Write the Particular Solution

Substitute $A = 0$ and $B = \dfrac{1}{1000}$:

$$
y_p(t) = t \left( 0 \cdot \cos(5t) + \dfrac{1}{1000} \sin(5t) \right) = \dfrac{t}{1000} \sin(5t)
$$

### Form the General Solution

The general solution is:

$$
y(t) = y_h(t) + y_p(t) = C_1 \cos(5t) + C_2 \sin(5t) + \dfrac{t}{1000} \sin(5t)
$$

### Apply Initial Conditions

Given $y(0) = 0$ and $y'(0) = 0$:

1. **At $t = 0$:**

   $$
   y(0) = C_1 \cos(0) + C_2 \sin(0) + \dfrac{0}{1000} \sin(0) = C_1
   $$

   Since $y(0) = 0$:

   $$
   C_1 = 0
   $$

2. **First Derivative $y'(t)$:**

   $$
   \begin{aligned}
   y'(t) &= -5 C_1 \sin(5t) + 5 C_2 \cos(5t) + \dfrac{d}{dt} \left( \dfrac{t}{1000} \sin(5t) \right) \\
   &= 5 C_2 \cos(5t) + \dfrac{1}{1000} \sin(5t) + \dfrac{5t}{1000} \cos(5t)
   \end{aligned}
   $$

   **At $t = 0$:**

   $$
   y'(0) = 5 C_2 \cos(0) + \dfrac{1}{1000} \sin(0) + \dfrac{5 \cdot 0}{1000} \cos(0) = 5 C_2
   $$

   Since $y'(0) = 0$:

   $$
   C_2 = 0
   $$

### Final Solution

With $C_1 = 0$ and $C_2 = 0$, the solution simplifies to:

$$
y(t) = \dfrac{t}{1000} \sin(5t)
$$

:::

::: {.callout-note icon=false collapse="true"}
## **Problem**
Consider the initial-value problem for the undamped spring-mass system:

$$
y'' + 36 y = 2 e^{6t}
$$

with parameters:

- $m = 1$
- $k = 36$
- $F(t) = 2 e^{6t}$
- Initial conditions: $y(0) = 0$ and $y'(0) = 0$

Solve for $y(t)$, determine the maximum displacement, and state if resonance or beats are present.

:::

::: {.callout-tip icon=false collapse="true"}
## **Solution:**

### Solve the Homogeneous Equation

The homogeneous equation is:

$$
y_h'' + 36 y_h = 0
$$

The characteristic equation is:

$$
r^2 + 36 = 0 \quad \Rightarrow \quad r = \pm 6i
$$

The general solution to the homogeneous equation is:

$$
y_h(t) = C_1 \cos(6t) + C_2 \sin(6t)
$$

### Find the Particular Solution

The non-homogeneous term is $f(t) = 2 e^{6t}$. Since this is an exponential function and does not overlap with the homogeneous solution, assume a particular solution of the form:

$$
y_p(t) = A e^{6t}
$$

### Compute the Derivatives of $y_p(t)$

Calculate the first and second derivatives:

1. **First Derivative $y_p'(t)$:**

   $$
   y_p'(t) = 6 A e^{6t}
   $$

2. **Second Derivative $y_p''(t)$:**

   $$
   y_p''(t) = 36 A e^{6t}
   $$

### Substitute into the Original Equation

Substitute $y_p(t)$, $y_p'(t)$, and $y_p''(t)$ into the differential equation:

$$
y_p'' + 36 y_p = 2 e^{6t}
$$

Substitute the expressions:

$$
36 A e^{6t} + 36 A e^{6t} = 2 e^{6t}
$$

Simplify:

$$
72 A e^{6t} = 2 e^{6t}
$$

Divide both sides by $e^{6t}$:

$$
72 A = 2
$$

### Solve for $A$

$$
A = \dfrac{2}{72} = \dfrac{1}{36}
$$

### Write the Particular Solution

$$
y_p(t) = \dfrac{1}{36} e^{6t}
$$

### Form the General Solution

The general solution is:

$$
y(t) = y_h(t) + y_p(t) = C_1 \cos(6t) + C_2 \sin(6t) + \dfrac{1}{36} e^{6t}
$$

### Apply Initial Conditions

Given $y(0) = 0$ and $y'(0) = 0$, we can solve for $C_1$ and $C_2$.

1. **At $t = 0$:**

   $$
   y(0) = C_1 \cos(0) + C_2 \sin(0) + \dfrac{1}{36} e^{0} = C_1 + \dfrac{1}{36}
   $$
   
   Since $y(0) = 0$:

   $$
   C_1 + \dfrac{1}{36} = 0 \quad \Rightarrow \quad C_1 = -\dfrac{1}{36}
   $$

2. **First Derivative $y'(t)$:**

   Calculate $y'(t)$:

   $$
   y'(t) = -6 C_1 \sin(6t) + 6 C_2 \cos(6t) + \dfrac{1}{36} \cdot 6 e^{6t} = -6 C_1 \sin(6t) + 6 C_2 \cos(6t) + \dfrac{1}{6} e^{6t}
   $$

   At $t = 0$:

   $$
   y'(0) = -6 C_1 \sin(0) + 6 C_2 \cos(0) + \dfrac{1}{6} e^{0} = 6 C_2 + \dfrac{1}{6}
   $$

   Since $y'(0) = 0$:

   $$
   6 C_2 + \dfrac{1}{6} = 0 \quad \Rightarrow \quad C_2 = -\dfrac{1}{36}
   $$

### Write the Final Solution

Substitute $C_1 = -\dfrac{1}{36}$ and $C_2 = -\dfrac{1}{36}$:

$$
y(t) = -\dfrac{1}{36} \cos(6t) - \dfrac{1}{36} \sin(6t) + \dfrac{1}{36} e^{6t}
$$



### Final Answer

The solution to the initial-value problem is:

$$
y(t) = -\dfrac{1}{36} \cos(6t) - \dfrac{1}{36} \sin(6t) + \dfrac{1}{36} e^{6t}
$$

- **Resonance is not present** in this system.
- **Beats are not present**.
- **Maximum displacement** increases exponentially due to the term $\dfrac{1}{36} e^{6t}$.

:::

## **Higher-Order Homogeneous Differential Equation Problems**

::: {.callout-note icon=false collapse="true"}
## **Problem**
$$
y''' - 2y'' - y' + 2y = 0
$$

:::

::: {.callout-tip icon=false collapse="true"}
## **Solution:**

###  Write the Characteristic Equation
Since this is a third-order differential equation, the characteristic equation is:

$$
r^3 - 2r^2 - r + 2 = 0
$$

### Factor the Characteristic Polynomial

1. Testing $r = 1$:
   $$
   1^3 - 2(1)^2 - 1 + 2 = 1 - 2 - 1 + 2 = 0
   $$
   Since $r = 1$ is a root, factor $r - 1$ out of the polynomial.

2. Divide $r^3 - 2r^2 - r + 2$ by $r - 1$ using synthetic division or polynomial division:

   - Dividing $r^3 - 2r^2 - r + 2$ by $r - 1$:
     $$
     r^3 - 2r^2 - r + 2 = (r - 1)(r^2 - r - 2)
     $$

3. Factor $r^2 - r - 2$:
   $$
   r^2 - r - 2 = (r - 2)(r + 1)
   $$

The characteristic equation factors as:
$$
(r - 1)(r - 2)(r + 1) = 0
$$

### Solve for the Roots
The roots of the characteristic equation are:
$$
r = 1, \quad r = 2, \quad r = -1
$$

### Write the General Solution
Since all the roots are real and distinct, the general solution for $y(t)$ is:

$$
y(t) = C_1 e^{t} + C_2 e^{2t} + C_3 e^{-t}
$$

where $C_1$, $C_2$, and $C_3$ are constants determined by initial conditions.

### Final Answer
The general solution to the differential equation is:

$$
y(t) = C_1 e^{t} + C_2 e^{2t} + C_3 e^{-t}
$$

:::

::: {.callout-note icon=false collapse="true"}
## **Problem**
$$
y^{(4)} + 4y''' + 6y'' + 4y' + y = 0
$$

:::

::: {.callout-tip icon=false collapse="true"}
## **Solution:**

### Write the Characteristic Equation
For a differential equation of the form $y^{(4)} + 4y''' + 6y'' + 4y' + y = 0$, replace each derivative with powers of $r$, giving:

$$
r^4 + 4r^3 + 6r^2 + 4r + 1 = 0
$$

### Recognize the Binomial Expansion
Notice that the characteristic polynomial:

$$
r^4 + 4r^3 + 6r^2 + 4r + 1
$$

resembles the binomial expansion of $(r + 1)^4$, which expands to:

$$
(r + 1)^4 = r^4 + 4r^3 + 6r^2 + 4r + 1
$$

Rewrite the characteristic equation as:

$$
(r + 1)^4 = 0
$$

### Solve for the Roots
The equation $(r + 1)^4 = 0$ has a repeated root:

$$
r = -1
$$

with multiplicity 4.

### Write the General Solution
Since $r = -1$ is a root with multiplicity 4, the general solution is:

$$
y(t) = (C_1 + C_2 t + C_3 t^2 + C_4 t^3)e^{-t}
$$

where $C_1$, $C_2$, $C_3$, and $C_4$ are constants determined by initial conditions.

### Final Answer
$$
y(t) = (C_1 + C_2 t + C_3 t^2 + C_4 t^3)e^{-t}
$$

:::

## **Eigenvectors/Eigenvalues Problems**

::: {.callout-note icon=false collapse="true"}
## **Problem**


:::

::: {.callout-tip icon=false collapse="true"}
## **Solution:**

:::

::: {.callout-note icon=false collapse="true"}
## **Problem**


:::

::: {.callout-tip icon=false collapse="true"}
## **Solution:**

:::

## **Nonhomogeneous Second-Order Differential Equation Problems**

::: {.callout-note icon=false collapse="true"}
## **Problem**


:::

::: {.callout-tip icon=false collapse="true"}
## **Solution:**

:::

::: {.callout-note icon=false collapse="true"}
## **Problem**


:::

::: {.callout-tip icon=false collapse="true"}
## **Solution:**

:::

## **Variation of Parameters Problems**

::: {.callout-tip collapse="true"}
## **Formula**
**Theorem 4.4.2 - Variation of Parameters Method**

For the differential equation
$$
y'' + a_1 y' + a_0 y = f(t),
$$
where $f$ is continuous, assume that $y_1$ and $y_2$ are linearly independent solutions of the corresponding homogeneous equation
$$
y'' + a_1 y' + a_0 y = 0.
$$
Then, a particular solution to the non-homogeneous equation is $y_p = u_1 y_1 + u_2 y_2$, where $u_1$ and $u_2$ satisfy

$$
u_1 = \int \frac{y_2 f}{y_2 y_1' - y_1 y_2'} \, dt \quad \text{and} \quad u_2 = \int \frac{y_1 f}{y_1 y_2' - y_2 y_1'} \, dt.
$$

:::

::: {.callout-note icon=false collapse="true"}
## **Problem**
Solve the non-homogeneous linear differential equation:

$$
y'' - 2 y' + y = \dfrac{e^{t}}{t}, \quad t > 0
$$

using the **Variation of Parameters** method.

:::

::: {.callout-tip icon=false collapse="true"}
## **Solution:**

### Solve the Homogeneous Equation

First, find the general solution to the corresponding homogeneous equation:

$$
y'' - 2 y' + y = 0
$$

**Characteristic Equation:**

Replace $y''$ with $r^2$, $y'$ with $r$, and $y$ with 1:

$$
r^2 - 2 r + 1 = 0
$$

**Solve for $r$:**

Factor the quadratic equation:

$$
(r - 1)^2 = 0
$$

We have a **repeated root** at $r = 1$.

**General Solution to the Homogeneous Equation:**

For a repeated root $r = 1$, the general solution is:

$$
y_h(t) = C_1 e^{r t} + C_2 t e^{r t} = C_1 e^{t} + C_2 t e^{t}
$$

where $C_1$ and $C_2$ are arbitrary constants.


### Step 2: Identify $y_1(t)$ and $y_2(t)$

From the homogeneous solution, the linearly independent solutions are:

- $y_1(t) = e^{t}$
- $y_2(t) = t e^{t}$


### Compute the Wronskian $W(y_1, y_2)(t)$

The Wronskian is:

$$
W(y_1, y_2)(t) = y_1(t) y_2'(t) - y_1'(t) y_2(t)
$$

**Compute $y_1'(t)$ and $y_2'(t)$:**

- $y_1'(t) = e^{t}$
- $y_2'(t) = \dfrac{d}{dt} [ t e^{t} ] = e^{t} + t e^{t} = e^{t} (1 + t)$

**Compute the Wronskian:**

$$
\begin{aligned}
W(y_1, y_2)(t) &= y_1(t) y_2'(t) - y_1'(t) y_2(t) \\
&= e^{t} \cdot e^{t} (1 + t) - e^{t} \cdot t e^{t} \\
&= e^{2t} (1 + t) - e^{2t} t \\
&= e^{2t} (1 + t - t) \\
&= e^{2t}
\end{aligned}
$$

$$
W(y_1, y_2)(t) = e^{2t}
$$

### Compute $u_1(t)$ and $u_2(t)$

**Given:**

$$
u_1(t) = \int \dfrac{y_2(t) f(t)}{W(y_1, y_2)(t)} \, dt, \quad u_2(t) = -\int \dfrac{y_1(t) f(t)}{W(y_1, y_2)(t)} \, dt
$$

**Compute $u_1(t)$:**

$$
\begin{aligned}
u_1(t) &= \int \dfrac{y_2(t) f(t)}{W(y_1, y_2)(t)} \, dt \\
&= \int \dfrac{ t e^{t} \cdot \dfrac{e^{t}}{t} }{ e^{2t} } \, dt \\
&= \int \dfrac{ t e^{t} \cdot \dfrac{e^{t}}{t} }{ e^{2t} } \, dt \\
&= \int \dfrac{ e^{t} \cdot e^{t} }{ e^{2t} } \, dt \\
&= \int \dfrac{ e^{2t} }{ e^{2t} } \, dt \\
&= \int 1 \, dt \\
&= t + C_1
\end{aligned}
$$

**Compute $u_2(t)$:**

$$
\begin{aligned}
u_2(t) &= -\int \dfrac{ y_1(t) f(t) }{ W(y_1, y_2)(t) } \, dt \\
&= -\int \dfrac{ e^{t} \cdot \dfrac{e^{t}}{t} }{ e^{2t} } \, dt \\
&= -\int \dfrac{ e^{t} \cdot \dfrac{e^{t}}{t} }{ e^{2t} } \, dt \\
&= -\int \dfrac{ e^{2t} }{ t e^{2t} } \, dt \\
&= -\int \dfrac{1}{t} \, dt \\
&= -\ln |t| + C_2
\end{aligned}
$$

Since $t > 0$, drop the absolute value:

$$
u_2(t) = -\ln t + C_2
$$


### Construct the Particular Solution $y_p(t)$

The particular solution is:

$$
\begin{aligned}
y_p(t) &= u_1(t) y_1(t) + u_2(t) y_2(t) \\
&= [ t + C_1 ] \cdot e^{t} + [ -\ln t + C_2 ] \cdot t e^{t} \\
&= e^{t} \left( t + C_1 - t \ln t + C_2 t \right)
\end{aligned}
$$

Since the constants $C_1$ and $C_2$ will be absorbed into the homogeneous solution, we can set $C_1 = 0$ and $C_2 = 0$ for the particular solution:

$$
y_p(t) = e^{t} \left( t - t \ln t \right) = t e^{t} (1 - \ln t)
$$



### General Solution

$$
\begin{aligned}
y(t) &= y_h(t) + y_p(t) \\
&= C_1 e^{t} + C_2 t e^{t} + t e^{t} (1 - \ln t)
\end{aligned}
$$

Simplify the expression:

$$
y(t) = e^{t} \left[ C_1 + C_2 t + t (1 - \ln t) \right]
$$


### **Final Answer**

The general solution to the differential equation is:

$$
 y(t) = e^{t} \left[ C_1 + C_2 t + t (1 - \ln t) \right]
$$

:::

::: {.callout-note icon=false collapse="true"}
## **Problem**


:::

::: {.callout-tip icon=false collapse="true"}
## **Solution:**

:::

## **Mixing Problems**

::: {.callout-note icon=false collapse="true"}
## **Problem**


:::

::: {.callout-tip icon=false collapse="true"}
## **Solution:**

:::

::: {.callout-note icon=false collapse="true"}
## **Problem**


:::

::: {.callout-tip icon=false collapse="true"}
## **Solution:**

:::