---
title: 'HOMEWORK 07'
author: 'Nathan Lunceford'
format:
  html:
    self-contained: true
    page-layout: full
    toc: true
    toc-depth: 2
    toc-location: right
    number-sections: false
    html-math-method: katex
    code-fold: true
    code-summary: 'Show the code'
    code-overflow: wrap
    code-copy: hover
    code-tools:
      source: false
      toggle: true
      caption: See code
editor:
  render-on-save: true
---

# SECTION 3.6

::: {.callout-tip}

## **Assigned:** 2, 5, 11, 13

:::

::: {.callout-note icon=false collapse="true"}

## 3.6.2

### Problem:

Show by direct substitution that the given particular solution $\mathbf{x}_p$ is indeed a solution to the nonhomogeneous system of equations. Then determine the general solution.

$$
\mathbf{x}' = \begin{bmatrix} 1 & -2 \\ -2 & 1 \end{bmatrix} \mathbf{x} + \begin{bmatrix} e^{2t} \\ 0 \end{bmatrix}, \quad \mathbf{x}_p = e^{2t} \begin{bmatrix} -\frac{1}{3} \\ \frac{2}{3} \end{bmatrix}
$$

### Solution:

#### **Calculate $\mathbf{x}_p'$:**

Differentiate $\mathbf{x}_p = e^{2t} \begin{bmatrix} -\frac{1}{3} \\ \frac{2}{3} \end{bmatrix}$ with respect to $t$:

$$
\mathbf{x}_p' = \begin{bmatrix} -\frac{1}{3} \cdot 2 e^{2t} \\ \frac{2}{3} \cdot 2 e^{2t} \end{bmatrix} = \begin{bmatrix} -\frac{2}{3} e^{2t} \\ \frac{4}{3} e^{2t} \end{bmatrix}
$$

#### **Calculate $A \mathbf{x}_p$:**

Substitute $\mathbf{x}_p$ into $A \mathbf{x}_p$:

$$
A \mathbf{x}_p = \begin{bmatrix} 1 & -2 \\ -2 & 1 \end{bmatrix} \begin{bmatrix} -\frac{1}{3} e^{2t} \\ \frac{2}{3} e^{2t} \end{bmatrix}
$$

Performing the matrix multiplication:

$$
A \mathbf{x}_p = \begin{bmatrix} -\frac{1}{3} e^{2t} - \frac{4}{3} e^{2t} \\ \frac{2}{3} e^{2t} + \frac{2}{3} e^{2t} \end{bmatrix} = \begin{bmatrix} -\frac{5}{3} e^{2t} \\ \frac{4}{3} e^{2t} \end{bmatrix}
$$

#### **Add $\mathbf{b}$ to $A \mathbf{x}_p$:**

$$
A \mathbf{x}_p + \mathbf{b} = \begin{bmatrix} -\frac{5}{3} e^{2t} \\ \frac{4}{3} e^{2t} \end{bmatrix} + \begin{bmatrix} e^{2t} \\ 0 \end{bmatrix} = \begin{bmatrix} -\frac{2}{3} e^{2t} \\ \frac{4}{3} e^{2t} \end{bmatrix}
$$

#### **Verify that $\mathbf{x}_p' = A \mathbf{x}_p + \mathbf{b}$:**

Since:

$$
\mathbf{x}_p' = \begin{bmatrix} -\frac{2}{3} e^{2t} \\ \frac{4}{3} e^{2t} \end{bmatrix} = A \mathbf{x}_p + \mathbf{b},
$$

$\mathbf{x}_p$ is indeed a particular solution.

#### **Find the general solution:**

The general solution is given by $\mathbf{x} = \mathbf{x}_h + \mathbf{x}_p$, where $\mathbf{x}_h$ solves the homogeneous system $\mathbf{x}' = A \mathbf{x}$.

1. **Find the eigenvalues of $A$:**

   The matrix $A = \begin{bmatrix} 1 & -2 \\ -2 & 1 \end{bmatrix}$ has eigenvalues $\lambda_1 = 3$ and $\lambda_2 = -1$.

2. **Find the eigenvectors corresponding to $\lambda_1$ and $\lambda_2$:**

   - For $\lambda_1 = 3$: Solve $(A - 3I) \mathbf{v} = 0$.

     $$
     (A - 3I) = \begin{bmatrix} -2 & -2 \\ -2 & -2 \end{bmatrix}
     $$

     Setting up the system:

     $$
     -2v_1 - 2v_2 = 0
     $$

     This simplifies to $v_1 = -v_2$. So, one eigenvector for $\lambda_1 = 3$ is:

     $$
     \mathbf{v}_1 = \begin{bmatrix} 1 \\ -1 \end{bmatrix}
     $$

   - For $\lambda_2 = -1$: Solve $(A + I) \mathbf{v} = 0$.

     $$
     (A + I) = \begin{bmatrix} 2 & -2 \\ -2 & 2 \end{bmatrix}
     $$

     Setting up the system:

     $$
     2v_1 - 2v_2 = 0
     $$

     This simplifies to $v_1 = v_2$. So, one eigenvector for $\lambda_2 = -1$ is:

     $$
     \mathbf{v}_2 = \begin{bmatrix} 1 \\ 1 \end{bmatrix}
     $$

3. **Formulate the homogeneous solution:**

   The homogeneous solution is:

   $$
   \mathbf{x}_h = c_1 e^{3t} \begin{bmatrix} 1 \\ -1 \end{bmatrix} + c_2 e^{-t} \begin{bmatrix} 1 \\ 1 \end{bmatrix}
   $$

#### **Combine to get the general solution:**

$$
\mathbf{x} = c_1 e^{3t} \begin{bmatrix} 1 \\ -1 \end{bmatrix} + c_2 e^{-t} \begin{bmatrix} 1 \\ 1 \end{bmatrix} + e^{2t} \begin{bmatrix} -\frac{1}{3} \\ \frac{2}{3} \end{bmatrix}
$$

::: {.callout-tip icon=false}

## **Final Answer:**

$$
\mathbf{x} = c_1 e^{3t} \begin{bmatrix} 1 \\ -1 \end{bmatrix} + c_2 e^{-t} \begin{bmatrix} 1 \\ 1 \end{bmatrix} + e^{2t} \begin{bmatrix} -\frac{1}{3} \\ \frac{2}{3} \end{bmatrix}
$$

:::
:::

::: {.callout-note icon=false collapse="true"}

## 3.6.5

### **Problem:**

Consider the system of differential equations:

$$
\mathbf{x}' = \begin{bmatrix} 1 & 1 \\ 4 & 1 \end{bmatrix} \mathbf{x} + \begin{bmatrix} -1 \\ -3 \end{bmatrix}
$$

**(a)** Explain why it is reasonable to assume that $\mathbf{x}_p$ is a constant vector, and use this assumption to determine a particular solution to the given nonhomogeneous system.

**(b)** Determine the complementary solution $\mathbf{x}_h$ to the associated homogeneous system, $\mathbf{x}' = A \mathbf{x}$.

**(c)** State the general solution to the system.

**(d)** Is there an equilibrium solution to this system? If so, is it stable? Explain.

### **Solution:**

#### (a) **Finding a Particular Solution $\mathbf{x}_p$:**

It is reasonable to assume that $\mathbf{x}_p$ is a constant vector because the nonhomogeneous term $\begin{bmatrix} -1 \\ -3 \end{bmatrix}$ is a constant vector. Therefore, if $\mathbf{x}_p$ is a constant solution, then $\mathbf{x}_p' = 0$. Substitute $\mathbf{x}_p$ into the differential equation:

$$
0 = \begin{bmatrix} 1 & 1 \\ 4 & 1 \end{bmatrix} \mathbf{x}_p + \begin{bmatrix} -1 \\ -3 \end{bmatrix}
$$

Rearrange to solve for $\mathbf{x}_p$:

$$
\begin{bmatrix} 1 & 1 \\ 4 & 1 \end{bmatrix} \mathbf{x}_p = \begin{bmatrix} 1 \\ 3 \end{bmatrix}
$$

Let $\mathbf{x}_p = \begin{bmatrix} x_1 \\ x_2 \end{bmatrix}$. Then we have the system:

$$
\begin{cases} x_1 + x_2 = 1 \\ 4x_1 + x_2 = 3 \end{cases}
$$

Solving these equations:

1. From the first equation, $x_2 = 1 - x_1$.
2. Substitute $x_2 = 1 - x_1$ into the second equation:

   $$
   4x_1 + (1 - x_1) = 3
   $$

   Simplify:

   $$
   3x_1 = 2 \implies x_1 = \frac{2}{3}
   $$

3. Substitute $x_1 = \frac{2}{3}$ into $x_2 = 1 - x_1$:

   $$
   x_2 = 1 - \frac{2}{3} = \frac{1}{3}
   $$

A particular solution is:

$$
\mathbf{x}_p = \begin{bmatrix} \frac{2}{3} \\ \frac{1}{3} \end{bmatrix}
$$

#### (b) **Finding the Complementary Solution $\mathbf{x}_h$:**

To find the complementary solution, solve the associated homogeneous system:

$$
\mathbf{x}' = \begin{bmatrix} 1 & 1 \\ 4 & 1 \end{bmatrix} \mathbf{x}
$$

1. **Find the eigenvalues of $A = \begin{bmatrix} 1 & 1 \\ 4 & 1 \end{bmatrix}$:**

   The characteristic polynomial is:

   $$
   \det(A - \lambda I) = \begin{vmatrix} 1 - \lambda & 1 \\ 4 & 1 - \lambda \end{vmatrix} = (\lambda - 1)^2 - 4 = \lambda^2 - 2\lambda - 3 = 0
   $$

   Solving for $\lambda$:

   $$
   \lambda^2 - 2\lambda - 3 = 0 \implies (\lambda - 3)(\lambda + 1) = 0
   $$

   So, the eigenvalues are $\lambda_1 = 3$ and $\lambda_2 = -1$.

2. **Find the eigenvectors for each eigenvalue:**

   - For $\lambda_1 = 3$:

     Solve $(A - 3I) \mathbf{v} = 0$:

     $$
     \begin{bmatrix} -2 & 1 \\ 4 & -2 \end{bmatrix} \begin{bmatrix} v_1 \\ v_2 \end{bmatrix} = 0
     $$

     This simplifies to $v_1 = \frac{1}{2} v_2$. An eigenvector corresponding to $\lambda_1 = 3$ is:

     $$
     \mathbf{v}_1 = \begin{bmatrix} 1 \\ 2 \end{bmatrix}
     $$

   - For $\lambda_2 = -1$:

     Solve $(A + I) \mathbf{v} = 0$:

     $$
     \begin{bmatrix} 2 & 1 \\ 4 & 2 \end{bmatrix} \begin{bmatrix} v_1 \\ v_2 \end{bmatrix} = 0
     $$

     This simplifies to $v_1 = -\frac{1}{2} v_2$. An eigenvector corresponding to $\lambda_2 = -1$ is:

     $$
     \mathbf{v}_2 = \begin{bmatrix} -1 \\ 2 \end{bmatrix}
     $$

3. **Formulate the complementary solution:**

   $$
   \mathbf{x}_h = c_1 e^{3t} \begin{bmatrix} 1 \\ 2 \end{bmatrix} + c_2 e^{-t} \begin{bmatrix} -1 \\ 2 \end{bmatrix}
   $$

#### (c) **State the General Solution:**

$$
\mathbf{x} = \mathbf{x}_h + \mathbf{x}_p = c_1 e^{3t} \begin{bmatrix} 1 \\ 2 \end{bmatrix} + c_2 e^{-t} \begin{bmatrix} -1 \\ 2 \end{bmatrix} + \begin{bmatrix} \frac{2}{3} \\ \frac{1}{3} \end{bmatrix}
$$

#### (d) **Equilibrium Solution and Stability:**

An equilibrium solution $\mathbf{x}_{\text{eq}}$ occurs when $\mathbf{x}' = 0$. This is satisfied by the particular solution $\mathbf{x}_p = \begin{bmatrix} \frac{2}{3} \\ \frac{1}{3} \end{bmatrix}$. Thus, $\mathbf{x}_{\text{eq}} = \mathbf{x}_p$.

To determine stability, look at the eigenvalues of $A$. Since one eigenvalue ($\lambda_1 = 3$) is positive and the other ($\lambda_2 = -1$) is negative, the equilibrium point is a **saddle point** and is therefore **unstable**.

::: {.callout-tip icon=false}

## **Final Answer:**

**(a)** Particular solution: $\mathbf{x}_p = \begin{bmatrix} \frac{2}{3} \\ \frac{1}{3} \end{bmatrix}$

**(b)** Complementary solution: $\mathbf{x}_h = c_1 e^{3t} \begin{bmatrix} 1 \\ 2 \end{bmatrix} + c_2 e^{-t} \begin{bmatrix} -1 \\ 2 \end{bmatrix}$

**(c)** General solution:

$$
\mathbf{x} = c_1 e^{3t} \begin{bmatrix} 1 \\ 2 \end{bmatrix} + c_2 e^{-t} \begin{bmatrix} -1 \\ 2 \end{bmatrix} + \begin{bmatrix} \frac{2}{3} \\ \frac{1}{3} \end{bmatrix}
$$

**(d)** Equilibrium solution: $\mathbf{x}_{\text{eq}} = \begin{bmatrix} \frac{2}{3} \\ \frac{1}{3} \end{bmatrix}$, which is unstable (saddle point).

:::
:::

::: {.callout-note icon=false collapse="true"}

## 3.6.11

### **Problem:**

Consider the system of differential equations:

$$
\mathbf{x}' = \begin{bmatrix} -1 & 1 \\ 0 & 1 \end{bmatrix} \mathbf{x} + \begin{bmatrix} 3e^{-2t} \\ -4e^{-2t} \end{bmatrix}
$$

**(a)** Assume an appropriate form for the particular solution $\mathbf{x}_p$ and use this assumption to determine a particular solution to the given nonhomogeneous system.

**(b)** Determine the complementary solution $\mathbf{x}_h$ to the associated homogeneous system, $\mathbf{x}' = A \mathbf{x}$.

**(c)** State the general solution to the system.

### **Solution:**

#### (a) **Finding a Particular Solution $\mathbf{x}_p$:**

The nonhomogeneous term is $\mathbf{b} = \begin{bmatrix} 3e^{-2t} \\ -4e^{-2t} \end{bmatrix}$. Since $e^{-2t}$ is not a solution to the homogeneous system (verified in part **(b)**), assume a particular solution of the form:

$$
\mathbf{x}_p(t) = \begin{bmatrix} a_1 \\ a_2 \end{bmatrix} e^{-2t}
$$

where $a_1$ and $a_2$ are constants to be determined.

**Differentiate $\mathbf{x}_p$:**

If $\mathbf{x}_p = \begin{bmatrix} a_1 \\ a_2 \end{bmatrix} e^{-2t}$, then:

$$
\mathbf{x}'_p = \begin{bmatrix} a_1 \\ a_2 \end{bmatrix} (-2e^{-2t}) = \begin{bmatrix} -2a_1 \\ -2a_2 \end{bmatrix} e^{-2t}
$$

**Substitute $\mathbf{x}_p$ and $\mathbf{x}'_p$ into the differential equation:**

We substitute $\mathbf{x}'_p$ and $A\mathbf{x}_p + \mathbf{f}(t)$ into the equation:

$$
\begin{bmatrix} -2a_1 \\ -2a_2 \end{bmatrix} e^{-2t} = \begin{bmatrix} -1 & 1 \\ 0 & 1 \end{bmatrix} \begin{bmatrix} a_1 \\ a_2 \end{bmatrix} e^{-2t} + \begin{bmatrix} 3 \\ -4 \end{bmatrix} e^{-2t}
$$

Expanding the matrix multiplication:

$$
\begin{bmatrix} -2a_1 \\ -2a_2 \end{bmatrix} e^{-2t} = \begin{bmatrix} -a_1 + a_2 \\ a_2 \end{bmatrix} e^{-2t} + \begin{bmatrix} 3 \\ -4 \end{bmatrix} e^{-2t}
$$

**Set up and solve the system of equations:**

1. $-2a_1 = -a_1 + a_2 + 3$
2. $-2a_2 = a_2 - 4$

- From the second equation: $-2a_2 = a_2 - 4 \Rightarrow -3a_2 = -4 \Rightarrow a_2 = \frac{4}{3}$.
- Substitute $a_2 = \frac{4}{3}$ into the first equation:

  $$
  -2a_1 = -a_1 + \frac{4}{3} + 3
  $$

  Simplifying:

  $$
  -a_1 = \frac{4}{3} + 3 \Rightarrow a_1 = -\frac{13}{3}
  $$

A particular solution is:

$$
\mathbf{x}_p(t) = \begin{bmatrix} -\frac{13}{3} \\ \frac{4}{3} \end{bmatrix} e^{-2t}
$$

#### (b) **Finding the Complementary Solution $\mathbf{x}_h$:**

**Solve the associated homogeneous system:**

$$
\mathbf{x}' = \begin{bmatrix} -1 & 1 \\ 0 & 1 \end{bmatrix} \mathbf{x}
$$

**Find the eigenvalues of $A = \begin{bmatrix} -1 & 1 \\ 0 & 1 \end{bmatrix}$:**

$$
\det(A - \lambda I) = \det \begin{bmatrix} -1 - \lambda & 1 \\ 0 & 1 - \lambda \end{bmatrix} = (-1 - \lambda)(1 - \lambda)
$$

$$
(-1 - \lambda)(1 - \lambda) = 0
$$

The eigenvalues are:

- $\lambda_1 = -1$
- $\lambda_2 = 1$

**Find the eigenvectors for each eigenvalue:**

- For $\lambda_1 = -1$:

  Solve $(A + I)\mathbf{v} = 0$:

  $$
  \begin{bmatrix} 0 & 1 \\ 0 & 2 \end{bmatrix} \begin{bmatrix} v_1 \\ v_2 \end{bmatrix} = \begin{bmatrix} 0 \\ 0 \end{bmatrix}
  $$

  This implies $v_2 = 0$, so $v_1$ is arbitrary. Choose $v_1 = 1$, giving:

  $$
  \mathbf{v}_1 = \begin{bmatrix} 1 \\ 0 \end{bmatrix}
  $$

- For $\lambda_2 = 1$:

  Solve $(A - I)\mathbf{v} = 0$:

  $$
  \begin{bmatrix} -2 & 1 \\ 0 & 0 \end{bmatrix} \begin{bmatrix} v_1 \\ v_2 \end{bmatrix} = \begin{bmatrix} 0 \\ 0 \end{bmatrix}
  $$

  This implies $v_1 = \frac{1}{2}v_2$ and $v_2$ is arbitrary. Choosing $v_2 = 2$:

  $$
  \mathbf{v}_2 = \begin{bmatrix} 1 \\ 2 \end{bmatrix}
  $$

**The complementary solution is:**

$$
\mathbf{x}_h(t) = c_1 e^{-t} \begin{bmatrix} 1 \\ 0 \end{bmatrix} + c_2 e^{t} \begin{bmatrix} 1 \\ 2 \end{bmatrix}
$$

#### (c) **State the General Solution:**

The general solution is the sum of the complementary solution $\mathbf{x}_h$ and the particular solution $\mathbf{x}_p$:

$$
\mathbf{x}(t) = \mathbf{x}_h + \mathbf{x}_p = c_1 e^{-t} \begin{bmatrix} 1 \\ 0 \end{bmatrix} + c_2 e^{t} \begin{bmatrix} 1 \\ 2 \end{bmatrix} + \begin{bmatrix} -\frac{13}{3} \\ \frac{4}{3} \end{bmatrix} e^{-2t}
$$

::: {.callout-tip icon=false}

## **Final Answer:**

**(a)** The particular solution is:

$$
\mathbf{x}_p(t) = \begin{bmatrix} -\frac{13}{3} \\ \frac{4}{3} \end{bmatrix} e^{-2t}
$$

**(b)** The complementary solution to the homogeneous system is:

$$
\mathbf{x}_h(t) = c_1 e^{-t} \begin{bmatrix} 1 \\ 0 \end{bmatrix} + c_2 e^{t} \begin{bmatrix} 1 \\ 2 \end{bmatrix}
$$

**(c)** The general solution to the system is:

$$
\mathbf{x}(t) = c_1 e^{-t} \begin{bmatrix} 1 \\ 0 \end{bmatrix} + c_2 e^{t} \begin{bmatrix} 1 \\ 2 \end{bmatrix} + \begin{bmatrix} -\frac{13}{3} \\ \frac{4}{3} \end{bmatrix} e^{-2t}
$$

:::
:::

::: {.callout-note icon=false collapse="true"}

## 3.6.13

### **Problem:**

Consider the system of differential equations:

$$
\mathbf{x}' = \begin{bmatrix} 0 & 1 \\ -1 & 0 \end{bmatrix} \mathbf{x} + \begin{bmatrix} 3 \\ -2 \end{bmatrix}
$$

**(a)** Assume an appropriate form for the particular solution $\mathbf{x}_p$ and use this assumption to determine a particular solution to the given nonhomogeneous system.

**(b)** Determine the complementary solution $\mathbf{x}_h$ to the associated homogeneous system, $\mathbf{x}' = A \mathbf{x}$.

**(c)** State the general solution to the system.

### **Solution:**

#### (a) **Finding a Particular Solution $\mathbf{x}_p$:**

The nonhomogeneous term is the constant vector $\mathbf{b} = \begin{bmatrix} 3 \\ -2 \end{bmatrix}$. Since it is a constant vector, we can assume a constant particular solution.

**Assume a particular solution of the form:**

$$
\mathbf{x}_p = \begin{bmatrix} a_1 \\ a_2 \end{bmatrix}
$$

where $a$ and $b$ are constants to be determined.

**Compute the derivative of $\mathbf{x}_p$:**

Since $\mathbf{x}_p$ is constant, its derivative is zero:

$$
\mathbf{x}'_p = \begin{bmatrix} 0 \\ 0 \end{bmatrix}
$$

**Substitute $\mathbf{x}_p$ and $\mathbf{x}'_p$ into the differential equation:**

$$
\mathbf{0} = A \mathbf{x}_p + \begin{bmatrix} 3 \\ -2 \end{bmatrix}
$$

Compute $A \mathbf{x}_p$:

$$
A \mathbf{x}_p = \begin{bmatrix} 0 & 1 \\ -1 & 0 \end{bmatrix} \begin{bmatrix} a_1 \\ a_2 \end{bmatrix} = \begin{bmatrix} a_2 \\ -a_1 \end{bmatrix}
$$

So the equation becomes:

$$
\begin{bmatrix} 0 \\ 0 \end{bmatrix} = \begin{bmatrix} a_2 \\ -a_1 \end{bmatrix} + \begin{bmatrix} 3 \\ -2 \end{bmatrix}
$$

**Set up the system of equations:**

1. $a_2 + 3 = 0$
2. $-a_1 - 2 = 0$

**Solve for $a_1$ and $a_2$:**

From equation 1:

$$
a_2 = -3
$$

From equation 2:

$$
-a_1 - 2 = 0 \quad \Rightarrow \quad a_1 = -2
$$

**A particular solution is:**

$$
\mathbf{x}_p = \begin{bmatrix} -2 \\ -3 \end{bmatrix}
$$

#### (b) **Finding the Complementary Solution $\mathbf{x}_h$:**

**Solve the associated homogeneous system:**

$$
\mathbf{x}' = A \mathbf{x} = \begin{bmatrix} 0 & 1 \\ -1 & 0 \end{bmatrix} \mathbf{x}
$$

**Find the eigenvalues of $A$:**

Compute the characteristic equation:

$$
\det(A - \lambda I) = \det \begin{bmatrix} -\lambda & 1 \\ -1 & -\lambda \end{bmatrix} = (-\lambda)(-\lambda) - (-1)(1) = \lambda^2 + 1
$$

Set the determinant to zero:

$$
\lambda^2 + 1 = 0 \quad \Rightarrow \quad \lambda^2 = -1 \quad \Rightarrow \quad \lambda = \pm i
$$

**Eigenvalues:**

- $\lambda_1 = i$
- $\lambda_2 = -i$

**Find the eigenvectors for each eigenvalue:**

- **For $\lambda = i$:**

Solve $(A - i I) \mathbf{v} = \mathbf{0}$:

$$
\left( \begin{bmatrix} 0 & 1 \\ -1 & 0 \end{bmatrix} - i \begin{bmatrix} 1 & 0 \\ 0 & 1 \end{bmatrix} \right) \mathbf{v} = \mathbf{0} \quad \Rightarrow \quad \begin{bmatrix} -i & 1 \\ -1 & -i \end{bmatrix} \begin{bmatrix} v_1 \\ v_2 \end{bmatrix} = \begin{bmatrix} 0 \\ 0 \end{bmatrix}
$$

This leads to the equations:

1. $-i v_1 + v_2 = 0$
2. $-v_1 - i v_2 = 0$

From equation 1:

$$
v_2 = i v_1
$$

Substitute $v_2$ into equation 2:

$$
- v_1 - i (i v_1) = 0 \quad \Rightarrow \quad - v_1 - i^2 v_1 = 0 \quad \Rightarrow \quad - v_1 - (-1) v_1 = 0 \quad \Rightarrow \quad - v_1 + v_1 = 0
$$

Which simplifies to $0 = 0$, confirming consistency.

**Thus, an eigenvector corresponding to $\lambda = i$ is:**

$$
\mathbf{v}_1 = \begin{bmatrix} 1 \\ i \end{bmatrix}
$$

- **For $\lambda = -i$:**

Similarly, we find the eigenvector:

$$
\mathbf{v}_2 = \begin{bmatrix} 1 \\ -i \end{bmatrix}
$$

**Express the solution in terms of real functions:**

To obtain real solutions, we use Euler's formula and consider the real and imaginary parts.

**Compute $e^{i t} \mathbf{v}_1$:**

$$
e^{i t} \begin{bmatrix} 1 \\ i \end{bmatrix} = (\cos t + i \sin t) \begin{bmatrix} 1 \\ i \end{bmatrix} = \begin{bmatrix} \cos t + i \sin t \\ i \cos t - \sin t \end{bmatrix}
$$

**Extract the real and imaginary parts:**

- **Real part:**

$$
\operatorname{Re} \left( e^{i t} \begin{bmatrix} 1 \\ i \end{bmatrix} \right) = \begin{bmatrix} \cos t \\ -\sin t \end{bmatrix}
$$

- **Imaginary part:**

$$
\operatorname{Im} \left( e^{i t} \begin{bmatrix} 1 \\ i \end{bmatrix} \right) = \begin{bmatrix} \sin t \\ \cos t \end{bmatrix}
$$

**Thus, the general solution to the homogeneous system is:**

$$
\mathbf{x}_h(t) = c_1 \begin{bmatrix} \cos t \\ -\sin t \end{bmatrix} + c_2 \begin{bmatrix} \sin t \\ \cos t \end{bmatrix}
$$

#### (c) **State the General Solution:**

The general solution is the sum of the complementary solution $\mathbf{x}_h$ and the particular solution $\mathbf{x}_p$:

$$
\mathbf{x}(t) = \mathbf{x}_h(t) + \mathbf{x}_p = c_1 \begin{bmatrix} \cos t \\ -\sin t \end{bmatrix} + c_2 \begin{bmatrix} \sin t \\ \cos t \end{bmatrix} + \begin{bmatrix} -2 \\ -3 \end{bmatrix}
$$

::: {.callout-tip icon=false}

## **Final Answer:**

**(a)** The particular solution is:

$$
\mathbf{x}_p = \begin{bmatrix} -2 \\ -3 \end{bmatrix}
$$

**(b)** The complementary solution to the homogeneous system is:

$$
\mathbf{x}_h(t) = c_1 \begin{bmatrix} \cos t \\ -\sin t \end{bmatrix} + c_2 \begin{bmatrix} \sin t \\ \cos t \end{bmatrix}
$$

**(c)** The general solution to the system is:

$$
\mathbf{x}(t) = c_1 \begin{bmatrix} \cos t \\ -\sin t \end{bmatrix} + c_2 \begin{bmatrix} \sin t \\ \cos t \end{bmatrix} + \begin{bmatrix} -2 \\ -3 \end{bmatrix}
$$

:::
:::

# SECTION 3.7

::: {.callout-tip}

## **Assigned:** 1, 5, 7, 11

:::

::: {.callout-note icon=false collapse="true"}

## 3.7.1

### **Problem:**

### **Solution:**

::: {.callout-tip icon=false}

## **Final Answer:**

:::
:::

::: {.callout-note icon=false collapse="true"}

## 3.7.5

### **Problem:**

### **Solution:**

::: {.callout-tip icon=false}

## **Final Answer:**

:::
:::

::: {.callout-note icon=false collapse="true"}

## 3.7.7

### **Problem:**

### **Solution:**

::: {.callout-tip icon=false}

## **Final Answer:**

:::
:::

::: {.callout-note icon=false collapse="true"}

## 3.7.11

### **Problem:**

### **Solution:**

::: {.callout-tip icon=false}

## **Final Answer:**

:::
:::

# SECTION 3.8

::: {.callout-tip}

## **Assigned:** 4, 5, 7, 11

:::

::: {.callout-note icon=false collapse="true"}

## 3.8.4

### **Problem:**

### **Solution:**

::: {.callout-tip icon=false}

## **Final Answer:**

:::
:::

::: {.callout-note icon=false collapse="true"}

## 3.8.5

### **Problem:**

### **Solution:**

::: {.callout-tip icon=false}

## **Final Answer:**

:::
:::

::: {.callout-note icon=false collapse="true"}

## 3.8.7

### **Problem:**

### **Solution:**

::: {.callout-tip icon=false}

## **Final Answer:**

:::
:::

::: {.callout-note icon=false collapse="true"}

## 3.8.11

### **Problem:**

### **Solution:**

::: {.callout-tip icon=false}

## **Final Answer:**

:::
:::
